started adding the interpolation based fault localization

gravy/src/org/gravy/faultlocalization/InfeasibleCodeFaultLocalization.java
@@ -1,0 +1,165 @@
+/**
+ * 
+ */
+package org.gravy.faultlocalization;
+
+import java.util.HashSet;
+import java.util.LinkedList;
+import java.util.Map.Entry;
+import java.util.Set;
+
+import org.gravy.prover.Prover;
+import org.gravy.prover.ProverExpr;
+import org.gravy.prover.ProverFactory;
+import org.gravy.prover.ProverResult;
+import org.gravy.verificationcondition.AbstractTransitionRelation;
+import org.gravy.verificationcondition.FaultLocalizationTransitionRelation;
+
+import boogie.controlflow.BasicBlock;
+import boogie.controlflow.CfgAxiom;
+import boogie.controlflow.CfgProcedure;
+
+/**
+ * @author schaef
+ *
+ */
+public class InfeasibleCodeFaultLocalization {
+
+	/**
+	 * Applies fault localization to a set of (not necessarily connected) infeasible blocks.
+	 * @param tr
+	 * @param infeasibleBlocks
+	 */
+	public static void localizeFaults(AbstractTransitionRelation tr, Set<BasicBlock> infeasibleBlocks) {
+		LinkedList<HashSet<BasicBlock>> components = findConnectedComponents(infeasibleBlocks);
+		for (HashSet<BasicBlock> cmp : components) {
+			localizeFault(tr, cmp);
+		}
+	}
+
+	
+	/**
+	 * Applies fault localization to a set of connected infeasible blocks
+	 * @param tr
+	 * @param component
+	 */
+	public static void localizeFault(AbstractTransitionRelation tr, Set<BasicBlock> component) {		
+		CfgProcedure slice = tr.getProcedure().computeSlice(getSubprog(component), tr.getProcedure().getRootNode());
+		
+		ProverFactory pf = new org.gravy.prover.princess.PrincessProverFactory();
+		Prover prover = pf.spawn();
+		prover.setConstructProofs(true);
+		FaultLocalizationTransitionRelation sliceTr = new FaultLocalizationTransitionRelation(slice, tr.getControlFlowFactory(), prover);
+		
+		int partition = 0;
+		
+//		prover.addAssertion(sliceTr.getEnsures());
+//	
+		for (Entry<CfgAxiom, ProverExpr> entry : sliceTr.getPreludeAxioms().entrySet()) {
+			prover.addAssertion(entry.getValue());
+		}
+		
+		
+		prover.addAssertion(sliceTr.getRequires());
+		
+		prover.setPartitionNumber(partition++);
+        
+        for (ProverExpr assertion : sliceTr.obligations) {
+            prover.addAssertion(assertion);
+            prover.setPartitionNumber(partition++);        	
+        }
+		
+		ProverResult res = prover.checkSat(true);
+		if (res!=ProverResult.Unsat) {
+			throw new RuntimeException("Fault Localization failed!");
+		}
+		
+
+        int[][] ordering = new int[partition][1];
+        for (int i=0; i<partition; i++) {
+                ordering[i][0] = i;
+        }               
+        
+
+        ProverExpr[] interpolants = prover.interpolate(ordering);
+
+        //debug code
+        {
+                System.err.println("#interpolants: "+ interpolants.length + " / #assertions:");
+                for (int i=0; i<partition-1; i++) {                        
+                		System.err.println("Assertion "+i+":"+sliceTr.pe2StmtMap.get(sliceTr.obligations.get(i)));
+                        System.err.println("\tInterpolant "+i+":"+interpolants[i]);
+                }
+        }
+        		
+		System.err.println("Check subprog " + res); 
+	}
+	
+	/**
+	 * Collect all blocks that must can reach or can be reached by
+	 * the elements in component 
+	 * @param component
+	 * @return
+	 */
+	private static Set<BasicBlock> getSubprog(Set<BasicBlock> component) {
+		HashSet<BasicBlock> result = new HashSet<BasicBlock>();
+		result.addAll(getNeighbors(component, true));
+		result.addAll(getNeighbors(component, false));
+		return result;
+	}
+	
+	private static Set<BasicBlock> getNeighbors(Set<BasicBlock> blocks, boolean forward) {
+		LinkedList<BasicBlock> todo = new LinkedList<BasicBlock>();
+		HashSet<BasicBlock> done = new HashSet<BasicBlock>();
+		todo.addAll(blocks);
+		while (!todo.isEmpty()) {
+			BasicBlock current = todo.pop();
+			done.add(current);
+			for (BasicBlock b : getNeighbors(current, forward)) {
+				if (!todo.contains(b) && !done.contains(b)) {
+					todo.add(b);
+				}
+			}
+		}
+		return done;
+	}
+	
+	private static Set<BasicBlock> getNeighbors(BasicBlock b, boolean forward) {
+		if (forward) return b.getSuccessors();
+		return b.getPredecessors();
+	}
+	
+	
+	private static LinkedList<HashSet<BasicBlock>> findConnectedComponents(Set<BasicBlock> blocks) {
+		LinkedList<HashSet<BasicBlock>> components = new LinkedList<HashSet<BasicBlock>>();
+		LinkedList<BasicBlock> allblocks = new LinkedList<BasicBlock>();
+		allblocks.addAll(blocks);
+		while (!allblocks.isEmpty()) {
+			HashSet<BasicBlock> subprog = new HashSet<BasicBlock>();
+			LinkedList<BasicBlock> todo = new LinkedList<BasicBlock>();
+			todo.add(allblocks.pop());			
+
+			while (!todo.isEmpty()) {
+				BasicBlock current = todo.pop();
+				allblocks.remove(current);
+				subprog.add(current);
+				for (BasicBlock b : current.getPredecessors()) {
+					if (!subprog.contains(b) && !todo.contains(b) && allblocks.contains(b)) {
+						todo.add(b);
+					}
+				}
+				for (BasicBlock b : current.getSuccessors()) {
+					if (!subprog.contains(b) && !todo.contains(b) && allblocks.contains(b)) {
+						todo.add(b);
+					}
+				}				
+			}		
+			if (subprog.size()>0) {
+				components.add(subprog);
+			}
+		}
+		return components;
+	}
+	
+
+}
