gravy/src/org/gravy/verificationcondition/FaultLocalizationTransitionRelation.java
@@ -1,0 +1,136 @@
+package org.gravy.verificationcondition;
+
+import java.util.HashSet;
+import java.util.LinkedList;
+import java.util.List;
+
+import org.gravy.prover.Prover;
+import org.gravy.prover.ProverExpr;
+
+import boogie.controlflow.AbstractControlFlowFactory;
+import boogie.controlflow.BasicBlock;
+import boogie.controlflow.CfgProcedure;
+import boogie.controlflow.expression.CfgExpression;
+import boogie.controlflow.util.HasseDiagram;
+import boogie.controlflow.util.PartialBlockOrderNode;
+
+/**
+ * @author schaef TODO: if we plan to do interprocedural analysis, we have to
+ *         change the way globals are handled here.
+ */
+public class FaultLocalizationTransitionRelation extends
+		AbstractTransitionRelation {
+
+	public LinkedList<ProverExpr> obligations = new LinkedList<ProverExpr>();
+	
+	
+	public FaultLocalizationTransitionRelation(CfgProcedure cfg,
+			AbstractControlFlowFactory cff, Prover p) {
+		super(cfg, cff, p);
+		makePrelude();
+
+		// create the ProverExpr for the precondition
+		ProverExpr[] prec = new ProverExpr[cfg.getRequires().size()];
+		int i = 0;
+		for (CfgExpression expr : cfg.getRequires()) {
+			prec[i] = this.expression2proverExpression(expr);
+			i++;
+		}
+		this.requires = this.prover.mkAnd(prec);
+
+		// create the ProverExpr for the precondition
+		ProverExpr[] post = new ProverExpr[cfg.getEnsures().size()];
+		i = 0;
+		for (CfgExpression expr : cfg.getEnsures()) {
+			post[i] = this.expression2proverExpression(expr);
+			i++;
+		}
+		this.ensures = this.prover.mkAnd(post);
+
+
+		lala(cfg);
+
+		finalizeAxioms();
+	}
+
+	private void lala(CfgProcedure cfg) {
+		HasseDiagram hd = new HasseDiagram(cfg);
+		PartialBlockOrderNode pon = hd.findNode(cfg.getRootNode());
+
+		
+		LinkedList<BasicBlock> todo = new LinkedList<BasicBlock>();
+		todo.add(cfg.getRootNode());
+		while (!todo.isEmpty()) {
+			BasicBlock current = todo.pop();
+			obligations.addAll(statements2proverExpression(current.getStatements()));
+			BasicBlock next = bar(current, pon.getElements());
+			if (next!=null) {
+				todo.add(next);
+			}
+		}
+		
+	}
+
+	private BasicBlock bar(BasicBlock b, HashSet<BasicBlock> mustpass ) {
+		this.lastMustPass = null;
+		if (b.getSuccessors().size()==1 ) {
+			BasicBlock next = b.getSuccessors().iterator().next();
+			if (mustpass.contains(next)) {
+				return next;
+			} else {
+				throw new RuntimeException("SNAP");
+			}
+		} else if (b.getSuccessors().size()>1 ) {
+			LinkedList<ProverExpr> succs = new LinkedList<ProverExpr>();			
+			for (BasicBlock next : b.getSuccessors()) {
+				succs.add(block2tr(next, mustpass));
+			}
+			obligations.add(this.prover.mkOr(succs.toArray(new ProverExpr[succs.size()])));			
+		}
+		return this.lastMustPass;
+	}
+
+	private BasicBlock lastMustPass = null;
+	
+	private ProverExpr block2tr(BasicBlock b, HashSet<BasicBlock> mustpass) {
+		
+		ProverExpr post;
+		
+		HashSet<BasicBlock> targets = new HashSet<BasicBlock>();
+		for (BasicBlock succ : b.getSuccessors()) {
+			if (!mustpass.contains(succ)) {
+				targets.add(succ);
+			} else {
+				if (this.lastMustPass==null) {
+					this.lastMustPass = succ;
+				} else {
+					if (succ!=lastMustPass) {
+						throw new RuntimeException("Damn");
+					}
+				}
+			}
+		}
+		
+		if (targets.size() == 0) {
+			post = this.prover.mkLiteral(true);
+		} else if (targets.size() == 1) {
+			post = block2tr(targets.iterator().next(), mustpass);
+		} else {
+			ProverExpr[] succs = new ProverExpr[targets.size()];
+			int i = 0;
+			for (BasicBlock next : targets) {
+				succs[i++] = block2tr(next, mustpass);
+			}
+			post = this.prover.mkOr(succs);
+		}
+		
+		List<ProverExpr> stmts = statements2proverExpression(b.getStatements());
+		stmts.add(post);
+		ProverExpr[] conj = stmts.toArray(new ProverExpr[stmts.size()]);
+
+		return this.prover.mkAnd(conj);
+	}
+	
+	
+
+}
