gravy/src/org/gravy/verificationcondition/TransitionRelation.java
@@ -3,7 +3,6 @@ package org.gravy.verificationcondition;
 import java.util.HashMap;
 import java.util.LinkedList;
 import java.util.List;
-import java.util.Map.Entry;
 
 import org.gravy.prover.Prover;
 import org.gravy.prover.ProverExpr;
@@ -21,19 +20,10 @@ import boogie.controlflow.expression.CfgExpression;
  */
 public class TransitionRelation extends AbstractTransitionRelation {
 
-//	protected ProverExpr expetionalReturnFlag = null;
-	
-	//TODO: this is a hack, like the creation
-	//of this variable in the constructor
-//	public ProverExpr getExpetionalReturnFlag() {
-//		return expetionalReturnFlag;
-//	}
-
-	
 	public TransitionRelation(CfgProcedure cfg, AbstractControlFlowFactory cff, Prover p) {
 		super(cfg, cff, p);
 		makePrelude();
-
+		
 		//create the ProverExpr for the precondition 
 		ProverExpr[] prec = new ProverExpr[cfg.getRequires().size()];
 		int i=0;
@@ -51,54 +41,16 @@ public class TransitionRelation extends AbstractTransitionRelation {
 			i++;
 		}
 		this.ensures = this.prover.mkAnd(post);
-		
-		
+				
 		//encode the forward reachability
 		ProverExpr firstok = block2transitionRelation(cfg.getRootNode(),
 				this.reachabilityVariables, this.proofObligations);
 		
 		//the proof obligation for root als must contain that the block variable for root is true		
 		this.proofObligations.get(cfg.getRootNode()).add(firstok);
-		//encode the backward reachability as described in the ICFEM'13 paper
-		for (Entry<BasicBlock, ProverExpr> entry : this.reachabilityVariables.entrySet()) {
-            BasicBlock b = entry.getKey();
-            ProverExpr v = entry.getValue();
 
-            if (b.getPredecessors().isEmpty())
-                // nothing to do for the root
-                continue;
-	
-            //now add an implication of the form
-            // b_i => \/_{j in pre}b_j
-            //to make sure that b_i is also forward reachable.
-            LinkedList<ProverExpr> targets = new LinkedList<ProverExpr>();						
-            //and this is the right part
-            for (BasicBlock pred : b.getPredecessors()) {
-            	if (this.reachabilityVariables.containsKey(pred) && !pred.returns) {
-            		//we have to check this, because with the alternative
-            		//return encoding, not all predecessors might be
-            		//reachable
-            		targets.add(this.reachabilityVariables.get(pred));
-            	}
-            }
-
-            ProverExpr bwdreach = this.prover.mkOr((ProverExpr[]) targets
-                                                     .toArray(new ProverExpr[targets.size()]));
-            
-            ProverExpr bwdobligation = this.prover.mkOr(this.prover.mkNot(v), bwdreach);
-          //now add the backward obligation to the proof obligation
-            this.proofObligations.get(b).add(bwdobligation);
-        }
-
-
-			
-			//TODO: compute postcondition and precondition
-		
-		finalizeAxioms();
-		
-	}
-
-	
+		finalizeAxioms();		
+	}	
 	
 	private ProverExpr block2transitionRelation(BasicBlock b,
 			HashMap<BasicBlock, ProverExpr> blockvars,
@@ -108,9 +60,7 @@ public class TransitionRelation extends AbstractTransitionRelation {
 		}
 
 		ProverExpr post;
-		if (b.getSuccessors().size() == 0 
-				//|| (org.joogie.Options.v().isOldStyleEncoding() && b.returns) 
-				) {
+		if (b.getSuccessors().size() == 0  ) {
 			post = this.prover.mkLiteral(true);
 		} else if (b.getSuccessors().size() == 1) {
 			post = block2transitionRelation(
