gravy/test/out.bpl
@@ -9,15 +9,23 @@ type intArrHeap_type = [ref][int]int;
 const unique $type : Field javaType;
 const unique $alloc : Field bool;
 const unique $null : ref;
-const { :sourceloc "/Users/schaef/git/jar2bpl/jar2bpl_test/regression/corner_cases/cc01/CornerCases01.java",-1,-1,-1,-1 } unique java.lang.Object : javaType extends  complete;
-const { :sourceloc "/Users/schaef/git/jar2bpl/jar2bpl_test/regression/corner_cases/cc01/CornerCases01.java",-1,-1,-1,-1 } unique CornerCases01 : javaType extends  unique java.lang.Object complete;
-const { :sourceloc "/Users/schaef/git/jar2bpl/jar2bpl_test/regression/corner_cases/cc01/CornerCases01.java",-1,-1,-1,-1 } unique java.io.Serializable : javaType extends  unique java.lang.Object complete;
-const { :sourceloc "/Users/schaef/git/jar2bpl/jar2bpl_test/regression/corner_cases/cc01/CornerCases01.java",-1,-1,-1,-1 } unique java.lang.Throwable : javaType extends  unique java.io.Serializable, unique java.lang.Object complete;
-const { :sourceloc "/Users/schaef/git/jar2bpl/jar2bpl_test/regression/corner_cases/cc01/CornerCases01.java",-1,-1,-1,-1 } unique java.lang.Exception : javaType extends  unique java.lang.Throwable complete;
-const { :sourceloc "/Users/schaef/git/jar2bpl/jar2bpl_test/regression/corner_cases/cc01/CornerCases01.java",-1,-1,-1,-1 } unique java.lang.RuntimeException : javaType extends  unique java.lang.Exception complete;
-const { :sourceloc "/Users/schaef/git/jar2bpl/jar2bpl_test/regression/corner_cases/cc01/CornerCases01.java",-1,-1,-1,-1 } unique java.lang.Iterable : javaType extends  unique java.lang.Object complete;
-const { :sourceloc "/Users/schaef/git/jar2bpl/jar2bpl_test/regression/corner_cases/cc01/CornerCases01.java",-1,-1,-1,-1 } unique java.util.Collection : javaType extends  unique java.lang.Iterable, unique java.lang.Object complete;
-const { :sourceloc "/Users/schaef/git/jar2bpl/jar2bpl_test/regression/corner_cases/cc01/CornerCases01.java",-1,-1,-1,-1 } unique java.util.List : javaType extends  unique java.lang.Object, unique java.util.Collection complete;
+const { :sourceloc "/Users/schaef/git/jar2bpl/jar2bpl_test/regression/true_positives/tp01/InfeasibleCode01.java",-1,-1,-1,-1 } unique java.lang.Object : javaType extends  complete;
+const { :sourceloc "/Users/schaef/git/jar2bpl/jar2bpl_test/regression/true_positives/tp01/InfeasibleCode01.java",-1,-1,-1,-1 } unique InfeasibleCode01 : javaType extends  unique java.lang.Object complete;
+const { :sourceloc "/Users/schaef/git/jar2bpl/jar2bpl_test/regression/true_positives/tp01/InfeasibleCode01.java",-1,-1,-1,-1 } unique java.lang.Appendable : javaType extends  unique java.lang.Object complete;
+const { :sourceloc "/Users/schaef/git/jar2bpl/jar2bpl_test/regression/true_positives/tp01/InfeasibleCode01.java",-1,-1,-1,-1 } unique java.lang.CharSequence : javaType extends  unique java.lang.Object complete;
+const { :sourceloc "/Users/schaef/git/jar2bpl/jar2bpl_test/regression/true_positives/tp01/InfeasibleCode01.java",-1,-1,-1,-1 } unique java.lang.AbstractStringBuilder : javaType extends  unique java.lang.CharSequence, unique java.lang.Appendable, unique java.lang.Object complete;
+const { :sourceloc "/Users/schaef/git/jar2bpl/jar2bpl_test/regression/true_positives/tp01/InfeasibleCode01.java",-1,-1,-1,-1 } unique java.io.Serializable : javaType extends  unique java.lang.Object complete;
+const { :sourceloc "/Users/schaef/git/jar2bpl/jar2bpl_test/regression/true_positives/tp01/InfeasibleCode01.java",-1,-1,-1,-1 } unique java.lang.StringBuffer : javaType extends  unique java.lang.AbstractStringBuilder, unique java.io.Serializable, unique java.lang.CharSequence complete;
+const { :sourceloc "/Users/schaef/git/jar2bpl/jar2bpl_test/regression/true_positives/tp01/InfeasibleCode01.java",-1,-1,-1,-1 } unique java.lang.Comparable : javaType extends  unique java.lang.Object complete;
+const { :sourceloc "/Users/schaef/git/jar2bpl/jar2bpl_test/regression/true_positives/tp01/InfeasibleCode01.java",-1,-1,-1,-1 } unique java.lang.String : javaType extends  unique java.lang.Comparable, unique java.io.Serializable, unique java.lang.CharSequence, unique java.lang.Object complete;
+const unique $StringConst0 : ref extends  complete;
+const { :sourceloc "/Users/schaef/git/jar2bpl/jar2bpl_test/regression/true_positives/tp01/InfeasibleCode01.java",-1,-1,-1,-1 } unique java.lang.AutoCloseable : javaType extends  unique java.lang.Object complete;
+const { :sourceloc "/Users/schaef/git/jar2bpl/jar2bpl_test/regression/true_positives/tp01/InfeasibleCode01.java",-1,-1,-1,-1 } unique java.io.Closeable : javaType extends  unique java.lang.AutoCloseable, unique java.lang.Object complete;
+const { :sourceloc "/Users/schaef/git/jar2bpl/jar2bpl_test/regression/true_positives/tp01/InfeasibleCode01.java",-1,-1,-1,-1 } unique java.io.Flushable : javaType extends  unique java.lang.Object complete;
+const { :sourceloc "/Users/schaef/git/jar2bpl/jar2bpl_test/regression/true_positives/tp01/InfeasibleCode01.java",-1,-1,-1,-1 } unique java.io.OutputStream : javaType extends  unique java.io.Closeable, unique java.io.Flushable, unique java.lang.Object complete;
+const { :sourceloc "/Users/schaef/git/jar2bpl/jar2bpl_test/regression/true_positives/tp01/InfeasibleCode01.java",-1,-1,-1,-1 } unique java.io.FilterOutputStream : javaType extends  unique java.io.OutputStream complete;
+const { :sourceloc "/Users/schaef/git/jar2bpl/jar2bpl_test/regression/true_positives/tp01/InfeasibleCode01.java",-1,-1,-1,-1 } unique java.io.PrintStream : javaType extends  unique java.io.Closeable, unique java.io.FilterOutputStream, unique java.lang.Appendable complete;
+const unique $StringConst1 : ref extends  complete;
 var $heap : $heap_type;
 var $intArrayType : javaType;
 var $charArrayType : javaType;
@@ -30,6 +38,8 @@ var $boolArrHeap : boolArrHeap_type;
 var $refArrHeap : refArrHeap_type;
 var $realArrHeap : realArrHeap_type;
 var $intArrHeap : intArrHeap_type;
+var InfeasibleCode01$InfeasibleCode01$bases234 : Field ref;
+var java.io.PrintStream$java.lang.System$err237 : ref;
 function $arrayType(t:javaType) returns ($ret:javaType);
 function $intToReal(x:int) returns ($ret:real);
 function $intToBool(x:int) returns ($ret:bool) { (if x == 0 then false else true) }
@@ -46,516 +56,567 @@ function $shlInt(x:int, y:int) returns ($ret:int);
 function $ushrInt(x:int, y:int) returns ($ret:int);
 function $shrInt(x:int, y:int) returns ($ret:int);
 axiom (forall t : javaType :: $heap[$null,$type] <: t);
-procedure $new(obj_type:javaType) returns ($obj:ref);    ensures $heap[$obj,$alloc] == true;    requires $heap[$obj,$alloc] == false;    ensures $heap[$obj,$type] == obj_type;        ensures $obj != $null;
+procedure $new(obj_type:javaType) returns ($obj:ref);    ensures $heap[$obj,$alloc] == true;    requires $heap[$obj,$alloc] == false;    ensures $obj != $null;    ensures $heap[$obj,$type] == obj_type;    
 
-procedure java.lang.Object$java.lang.Object$clone$43($this:ref) returns ($other:ref);        ensures $heap[$other,$type] == $heap[$this,$type];    ensures $heap[$other,$alloc] == true;    ensures $other != $null;
+procedure java.lang.Object$java.lang.Object$clone$43($this:ref) returns ($other:ref);    ensures $heap[$other,$alloc] == true;    ensures $other != $null;        ensures $heap[$other,$type] == $heap[$this,$type];
 
 procedure int$java.lang.String$compareTo$87($this:ref, $other:ref) returns ($return:int);    
 
-procedure void$CornerCases01$decideCondition$1889($this:ref, $in_parameter__0:int, $in_parameter__1:int) returns ($exception:ref);    
+procedure boolean$InfeasibleCode01$foo$1889($this:ref, $in_parameter__0:ref) returns ($return:int, $exception:ref);    
 
-procedure void$java.lang.RuntimeException$$la$init$ra$$922($this:ref) returns ($exception:ref);    
+procedure int$java.lang.Object$hashCode$41($this:ref) returns ($return:int, $exception:ref);    
 
-procedure int$CornerCases01$decisions$1890($this:ref, $in_parameter__0:int, $in_parameter__1:int) returns ($return:int, $exception:ref);    
+procedure int$InfeasibleCode01$infeasible0$1890($this:ref, $in_parameter__0:ref) returns ($return:int, $exception:ref);    modifies $intArrHeap;
 
-procedure int$CornerCases01$getNewIndex$1891($this:ref, $in_parameter__0:int, $in_parameter__1:ref, $in_parameter__2:ref, $in_parameter__3:ref, $in_parameter__4:ref) returns ($return:int, $exception:ref);    modifies $heap;
+procedure int$InfeasibleCode01$infeasible1$1891($this:ref, $in_parameter__0:ref) returns ($return:int, $exception:ref);    
 
-procedure int$java.util.List$size$152($this:ref) returns ($return:int, $exception:ref);    modifies $heap;
+procedure void$java.lang.StringBuffer$$la$init$ra$$685($this:ref) returns ($exception:ref);    
 
-procedure int$CornerCases01$getInt$1892($this:ref, $in_parameter__0:int) returns ($return:int, $exception:ref);    
+procedure java.lang.String$java.lang.Object$toString$44($this:ref) returns ($return:ref, $exception:ref);    
 
-procedure void$CornerCases01$$la$init$ra$$1893($this:ref) returns ($exception:ref);    
+procedure java.lang.StringBuffer$java.lang.StringBuffer$append$701($this:ref, $in_parameter__0:ref) returns ($return:ref, $exception:ref);    
+
+procedure java.lang.String$java.lang.StringBuffer$toString$738($this:ref) returns ($return:ref, $exception:ref);    
+
+procedure void$java.io.PrintStream$println$217($this:ref, $in_parameter__0:ref) returns ($exception:ref);    
+
+procedure void$InfeasibleCode01$infeasible2$1892($this:ref, $in_parameter__0:ref) returns ($exception:ref);    modifies $intArrHeap;
+
+procedure void$InfeasibleCode01$infeasible3$1893($this:ref, $in_parameter__0:int, $in_parameter__1:int) returns ($exception:ref);    
+
+procedure boolean$InfeasibleCode01$infeasible4$1894($this:ref, $in_parameter__0:ref) returns ($return:int, $exception:ref);    
+
+procedure void$InfeasibleCode01$infeasible5$1895($this:ref) returns ($exception:ref);    modifies $stringSizeHeap;
+
+procedure int$InfeasibleCode01$infeasible6$1896($this:ref, $in_parameter__0:ref) returns ($return:int, $exception:ref);    
+
+procedure void$InfeasibleCode01$infeasible07$1897($this:ref, $in_parameter__0:ref) returns ($exception:ref);    
+
+procedure void$InfeasibleCode01$$la$init$ra$$1898($this:ref) returns ($exception:ref);    
 
 procedure void$java.lang.Object$$la$init$ra$$38($this:ref) returns ($exception:ref);    
 
-implementation void$CornerCases01$decideCondition$1889($this:ref, $in_parameter__0:int, $in_parameter__1:int) returns ($exception:ref){
+implementation boolean$InfeasibleCode01$foo$1889($this:ref, $in_parameter__0:ref) returns ($return:int, $exception:ref){
     
-var $fakelocal_0 : ref;    
-var temp$04 : ref;    
-var this1 : ref;    
-var notEqual3 : int;    
-var truthValue2 : int;
-    assume { :sourceloc "/Users/schaef/git/jar2bpl/jar2bpl_test/regression/corner_cases/cc01/CornerCases01.java",-1,-1,-1,-1 } $this != $null;
-    assert { :sourceloc "/Users/schaef/git/jar2bpl/jar2bpl_test/regression/corner_cases/cc01/CornerCases01.java",10,2,25,2 } true;
+var temp$03 : ref;    
+var temp$36 : ref;    
+var other2 : ref;    
+var temp$25 : int;    
+var temp$69 : int;    
+var temp$811 : int;    
+var temp$14 : ref;    
+var temp$710 : int;    
+var temp$58 : ref;    
+var temp$47 : int;    
+var this1 : ref;
+    assume { :sourceloc "/Users/schaef/git/jar2bpl/jar2bpl_test/regression/true_positives/tp01/InfeasibleCode01.java",-1,-1,-1,-1 } $this != $null;
+    assume $heap[$in_parameter__0,$type] <: InfeasibleCode01;
+    assert { :sourceloc "/Users/schaef/git/jar2bpl/jar2bpl_test/regression/true_positives/tp01/InfeasibleCode01.java",10,2,24,2 } true;
     this1 := $this;
-    assert { :sourceloc "/Users/schaef/git/jar2bpl/jar2bpl_test/regression/corner_cases/cc01/CornerCases01.java",10,30,10,43 } true;
-    truthValue2 := $in_parameter__0;
-    assert { :sourceloc "/Users/schaef/git/jar2bpl/jar2bpl_test/regression/corner_cases/cc01/CornerCases01.java",10,46,10,61 } true;
-    notEqual3 := $in_parameter__1;
-    assert { :sourceloc "/Users/schaef/git/jar2bpl/jar2bpl_test/regression/corner_cases/cc01/CornerCases01.java",14,7,14,14 } true;
-    if (notEqual3 == 0) {
-        assert { :sourceloc "/Users/schaef/git/jar2bpl/jar2bpl_test/regression/corner_cases/cc01/CornerCases01.java",15,4,15,10 } true;
+    assert { :sourceloc "/Users/schaef/git/jar2bpl/jar2bpl_test/regression/true_positives/tp01/InfeasibleCode01.java",10,14,10,35 } true;
+    other2 := $in_parameter__0;
+    assert { :sourceloc "/Users/schaef/git/jar2bpl/jar2bpl_test/regression/true_positives/tp01/InfeasibleCode01.java",11,7,11,11 } true;
+    temp$03 := $heap[this1,InfeasibleCode01$InfeasibleCode01$bases234];
+    assert { :sourceloc "/Users/schaef/git/jar2bpl/jar2bpl_test/regression/true_positives/tp01/InfeasibleCode01.java",11,7,11,11 } true;
+    if (temp$03 == $null) {
+        assert { :sourceloc "/Users/schaef/git/jar2bpl/jar2bpl_test/regression/true_positives/tp01/InfeasibleCode01.java",12,8,12,26 } { :comment "thenblock" } true;
         goto block1;
     }
-    assert { :sourceloc "/Users/schaef/git/jar2bpl/jar2bpl_test/regression/corner_cases/cc01/CornerCases01.java",14,7,14,14 } true;
+    assert { :sourceloc "/Users/schaef/git/jar2bpl/jar2bpl_test/regression/true_positives/tp01/InfeasibleCode01.java",12,8,12,26 } { :comment "elseblock" } true;
+    assert { :sourceloc "/Users/schaef/git/jar2bpl/jar2bpl_test/regression/true_positives/tp01/InfeasibleCode01.java",11,7,11,11 } true;
     goto block2;
-  block2:
-    assert { :sourceloc "/Users/schaef/git/jar2bpl/jar2bpl_test/regression/corner_cases/cc01/CornerCases01.java",14,7,14,14 } true;
-    assert { :sourceloc "/Users/schaef/git/jar2bpl/jar2bpl_test/regression/corner_cases/cc01/CornerCases01.java",14,19,14,33 } true;
-    if (truthValue2 == 0) {
-        assert { :sourceloc "/Users/schaef/git/jar2bpl/jar2bpl_test/regression/corner_cases/cc01/CornerCases01.java",14,19,14,33 } true;
+  block1:
+    assert { :sourceloc "/Users/schaef/git/jar2bpl/jar2bpl_test/regression/true_positives/tp01/InfeasibleCode01.java",12,8,12,26 } true;
+    assert { :sourceloc "/Users/schaef/git/jar2bpl/jar2bpl_test/regression/true_positives/tp01/InfeasibleCode01.java",12,8,12,26 } other2 != $null;
+    temp$14 := $heap[other2,InfeasibleCode01$InfeasibleCode01$bases234];
+    assert { :sourceloc "/Users/schaef/git/jar2bpl/jar2bpl_test/regression/true_positives/tp01/InfeasibleCode01.java",12,8,12,26 } true;
+    if (temp$14 != $null) {
+        assert { :sourceloc "/Users/schaef/git/jar2bpl/jar2bpl_test/regression/true_positives/tp01/InfeasibleCode01.java",12,8,12,26 } { :comment "thenblock" } true;
         goto block3;
     }
-    assert { :sourceloc "/Users/schaef/git/jar2bpl/jar2bpl_test/regression/corner_cases/cc01/CornerCases01.java",14,19,14,33 } true;
-    goto block1;
-    assert { :sourceloc "/Users/schaef/git/jar2bpl/jar2bpl_test/regression/corner_cases/cc01/CornerCases01.java",14,19,14,33 } true;
-    goto block3;
+    assert { :sourceloc "/Users/schaef/git/jar2bpl/jar2bpl_test/regression/true_positives/tp01/InfeasibleCode01.java",12,8,12,26 } { :comment "elseblock" } true;
+    assert { :sourceloc "/Users/schaef/git/jar2bpl/jar2bpl_test/regression/true_positives/tp01/InfeasibleCode01.java",12,8,12,26 } true;
+    goto block2;
   block3:
-    assert { :sourceloc "/Users/schaef/git/jar2bpl/jar2bpl_test/regression/corner_cases/cc01/CornerCases01.java",14,19,14,33 } true;
-    assert { :sourceloc "/Users/schaef/git/jar2bpl/jar2bpl_test/regression/corner_cases/cc01/CornerCases01.java",15,4,15,10 } true;
+    assert { :sourceloc "/Users/schaef/git/jar2bpl/jar2bpl_test/regression/true_positives/tp01/InfeasibleCode01.java",12,8,12,26 } true;
+    temp$25 := 0;
+    assert { :sourceloc "/Users/schaef/git/jar2bpl/jar2bpl_test/regression/true_positives/tp01/InfeasibleCode01.java",13,5,13,17 } true;
+    $return := temp$25;
     return;
-  block1:
-    assert { :sourceloc "/Users/schaef/git/jar2bpl/jar2bpl_test/regression/corner_cases/cc01/CornerCases01.java",15,4,15,10 } true;
-    assert { :sourceloc "/Users/schaef/git/jar2bpl/jar2bpl_test/regression/corner_cases/cc01/CornerCases01.java",16,14,16,21 } true;
-    if (notEqual3 == 0) {
-        assert { :sourceloc "/Users/schaef/git/jar2bpl/jar2bpl_test/regression/corner_cases/cc01/CornerCases01.java",18,4,18,10 } true;
+  block2:
+    assert { :sourceloc "/Users/schaef/git/jar2bpl/jar2bpl_test/regression/true_positives/tp01/InfeasibleCode01.java",16,7,16,11 } true;
+    temp$36 := $heap[this1,InfeasibleCode01$InfeasibleCode01$bases234];
+    assert { :sourceloc "/Users/schaef/git/jar2bpl/jar2bpl_test/regression/true_positives/tp01/InfeasibleCode01.java",16,7,16,11 } true;
+    assert { :sourceloc "/Users/schaef/git/jar2bpl/jar2bpl_test/regression/true_positives/tp01/InfeasibleCode01.java",16,7,16,11 } temp$36 != $null;
+    call temp$47, $exception := int$java.lang.Object$hashCode$41(temp$36);
+    assert { :sourceloc "/Users/schaef/git/jar2bpl/jar2bpl_test/regression/true_positives/tp01/InfeasibleCode01.java",16,7,16,11 } true;
+    assert { :sourceloc "/Users/schaef/git/jar2bpl/jar2bpl_test/regression/true_positives/tp01/InfeasibleCode01.java",16,7,16,11 } other2 != $null;
+    temp$58 := $heap[other2,InfeasibleCode01$InfeasibleCode01$bases234];
+    assert { :sourceloc "/Users/schaef/git/jar2bpl/jar2bpl_test/regression/true_positives/tp01/InfeasibleCode01.java",16,7,16,11 } true;
+    assert { :sourceloc "/Users/schaef/git/jar2bpl/jar2bpl_test/regression/true_positives/tp01/InfeasibleCode01.java",16,7,16,11 } temp$58 != $null;
+    call temp$69, $exception := int$java.lang.Object$hashCode$41(temp$58);
+    assert { :sourceloc "/Users/schaef/git/jar2bpl/jar2bpl_test/regression/true_positives/tp01/InfeasibleCode01.java",16,7,16,11 } true;
+    if (temp$47 != temp$69) {
+        assert { :sourceloc "/Users/schaef/git/jar2bpl/jar2bpl_test/regression/true_positives/tp01/InfeasibleCode01.java",16,7,16,11 } { :comment "thenblock" } true;
         goto block4;
     }
-    assert { :sourceloc "/Users/schaef/git/jar2bpl/jar2bpl_test/regression/corner_cases/cc01/CornerCases01.java",16,14,16,21 } true;
+    assert { :sourceloc "/Users/schaef/git/jar2bpl/jar2bpl_test/regression/true_positives/tp01/InfeasibleCode01.java",16,7,16,11 } { :comment "elseblock" } true;
+    assert { :sourceloc "/Users/schaef/git/jar2bpl/jar2bpl_test/regression/true_positives/tp01/InfeasibleCode01.java",16,7,16,11 } true;
     goto block5;
+  block4:
+    assert { :sourceloc "/Users/schaef/git/jar2bpl/jar2bpl_test/regression/true_positives/tp01/InfeasibleCode01.java",16,7,16,11 } true;
+    temp$710 := 0;
+    assert { :sourceloc "/Users/schaef/git/jar2bpl/jar2bpl_test/regression/true_positives/tp01/InfeasibleCode01.java",17,4,17,16 } true;
+    $return := temp$710;
+    return;
   block5:
-    assert { :sourceloc "/Users/schaef/git/jar2bpl/jar2bpl_test/regression/corner_cases/cc01/CornerCases01.java",16,14,16,21 } true;
-    assert { :sourceloc "/Users/schaef/git/jar2bpl/jar2bpl_test/regression/corner_cases/cc01/CornerCases01.java",16,26,16,40 } true;
-    if (truthValue2 == 1) {
-        assert { :sourceloc "/Users/schaef/git/jar2bpl/jar2bpl_test/regression/corner_cases/cc01/CornerCases01.java",16,26,16,40 } true;
+    assert { :sourceloc "/Users/schaef/git/jar2bpl/jar2bpl_test/regression/true_positives/tp01/InfeasibleCode01.java",17,4,17,16 } true;
+    temp$811 := 1;
+    assert { :sourceloc "/Users/schaef/git/jar2bpl/jar2bpl_test/regression/true_positives/tp01/InfeasibleCode01.java",23,3,23,14 } true;
+    $return := temp$811;
+    return;
+}
+
+
+implementation int$InfeasibleCode01$infeasible0$1890($this:ref, $in_parameter__0:ref) returns ($return:int, $exception:ref){
+    
+var temp$015 : ref;    
+var temp$318 : ref;    
+var temp$116 : int;    
+var temp$520 : int;    
+var this12 : ref;    
+var i14 : int;    
+var arr13 : ref;    
+var temp$419 : int;    
+var temp$217 : int;
+    assume { :sourceloc "/Users/schaef/git/jar2bpl/jar2bpl_test/regression/true_positives/tp01/InfeasibleCode01.java",-1,-1,-1,-1 } $this != $null;
+    assert { :sourceloc "/Users/schaef/git/jar2bpl/jar2bpl_test/regression/true_positives/tp01/InfeasibleCode01.java",27,2,31,2 } true;
+    this12 := $this;
+    assert { :sourceloc "/Users/schaef/git/jar2bpl/jar2bpl_test/regression/true_positives/tp01/InfeasibleCode01.java",27,25,27,33 } true;
+    arr13 := $in_parameter__0;
+    assert { :sourceloc "/Users/schaef/git/jar2bpl/jar2bpl_test/regression/true_positives/tp01/InfeasibleCode01.java",28,3,28,21 } true;
+    assert { :sourceloc "/Users/schaef/git/jar2bpl/jar2bpl_test/regression/true_positives/tp01/InfeasibleCode01.java",28,3,28,21 } arr13 != $null;
+    i14 := $arrSizeHeap[arr13];
+    assert { :sourceloc "/Users/schaef/git/jar2bpl/jar2bpl_test/regression/true_positives/tp01/InfeasibleCode01.java",29,3,29,11 } true;
+    temp$015 := arr13;
+    assert { :sourceloc "/Users/schaef/git/jar2bpl/jar2bpl_test/regression/true_positives/tp01/InfeasibleCode01.java",29,3,29,11 } true;
+    temp$116 := 3;
+    assert { :sourceloc "/Users/schaef/git/jar2bpl/jar2bpl_test/regression/true_positives/tp01/InfeasibleCode01.java",29,6,29,8 } true;
+    temp$217 := 3;
+    assert { :sourceloc "/Users/schaef/git/jar2bpl/jar2bpl_test/regression/true_positives/tp01/InfeasibleCode01.java",29,6,29,8 } true;
+    assert { :sourceloc "/Users/schaef/git/jar2bpl/jar2bpl_test/regression/true_positives/tp01/InfeasibleCode01.java",29,6,29,8 } temp$116 < $arrSizeHeap[temp$015] && temp$116 >= 0;
+    $intArrHeap := $intArrHeap[temp$015 := $intArrHeap[temp$015][temp$116 := temp$217]];
+    assert { :sourceloc "/Users/schaef/git/jar2bpl/jar2bpl_test/regression/true_positives/tp01/InfeasibleCode01.java",29,6,29,8 } true;
+    temp$318 := arr13;
+    assert { :sourceloc "/Users/schaef/git/jar2bpl/jar2bpl_test/regression/true_positives/tp01/InfeasibleCode01.java",29,6,29,8 } true;
+    temp$419 := i14;
+    assert { :sourceloc "/Users/schaef/git/jar2bpl/jar2bpl_test/regression/true_positives/tp01/InfeasibleCode01.java",29,6,29,8 } true;
+    assert { :sourceloc "/Users/schaef/git/jar2bpl/jar2bpl_test/regression/true_positives/tp01/InfeasibleCode01.java",29,6,29,8 } temp$419 < $arrSizeHeap[temp$318] && temp$419 >= 0;
+    temp$520 := $intArrHeap[temp$318][temp$419];
+    assert { :sourceloc "/Users/schaef/git/jar2bpl/jar2bpl_test/regression/true_positives/tp01/InfeasibleCode01.java",30,3,30,16 } true;
+    $return := temp$520;
+    return;
+}
+
+
+implementation int$InfeasibleCode01$infeasible1$1891($this:ref, $in_parameter__0:ref) returns ($return:int, $exception:ref){
+    
+var o22 : ref;    
+var $fakelocal_2 : ref;    
+var temp$225 : ref;    
+var temp$124 : ref;    
+var $fakelocal_1 : ref;    
+var this21 : ref;    
+var temp$528 : int;    
+var temp$023 : int;    
+var temp$427 : ref;    
+var $fakelocal_0 : ref;    
+var temp$326 : ref;
+    assume { :sourceloc "/Users/schaef/git/jar2bpl/jar2bpl_test/regression/true_positives/tp01/InfeasibleCode01.java",-1,-1,-1,-1 } $this != $null;
+    assume $heap[$in_parameter__0,$type] <: java.lang.Object;
+    assert { :sourceloc "/Users/schaef/git/jar2bpl/jar2bpl_test/regression/true_positives/tp01/InfeasibleCode01.java",33,2,39,2 } true;
+    this21 := $this;
+    assert { :sourceloc "/Users/schaef/git/jar2bpl/jar2bpl_test/regression/true_positives/tp01/InfeasibleCode01.java",33,25,33,32 } true;
+    o22 := $in_parameter__0;
+    assert { :sourceloc "/Users/schaef/git/jar2bpl/jar2bpl_test/regression/true_positives/tp01/InfeasibleCode01.java",34,7,34,13 } true;
+    if (o22 != $null) {
+        assert { :sourceloc "/Users/schaef/git/jar2bpl/jar2bpl_test/regression/true_positives/tp01/InfeasibleCode01.java",34,7,34,13 } { :comment "thenblock" } true;
         goto block6;
     }
-    assert { :sourceloc "/Users/schaef/git/jar2bpl/jar2bpl_test/regression/corner_cases/cc01/CornerCases01.java",16,26,16,40 } true;
-    goto block4;
-    assert { :sourceloc "/Users/schaef/git/jar2bpl/jar2bpl_test/regression/corner_cases/cc01/CornerCases01.java",16,26,16,40 } true;
-    goto block6;
+    assert { :sourceloc "/Users/schaef/git/jar2bpl/jar2bpl_test/regression/true_positives/tp01/InfeasibleCode01.java",34,7,34,13 } { :comment "elseblock" } true;
+    assert { :sourceloc "/Users/schaef/git/jar2bpl/jar2bpl_test/regression/true_positives/tp01/InfeasibleCode01.java",34,7,34,13 } true;
+    goto block7;
   block6:
-    assert { :sourceloc "/Users/schaef/git/jar2bpl/jar2bpl_test/regression/corner_cases/cc01/CornerCases01.java",16,26,16,40 } true;
-    assert { :sourceloc "/Users/schaef/git/jar2bpl/jar2bpl_test/regression/corner_cases/cc01/CornerCases01.java",18,4,18,10 } true;
+    assert { :sourceloc "/Users/schaef/git/jar2bpl/jar2bpl_test/regression/true_positives/tp01/InfeasibleCode01.java",34,7,34,13 } true;
+    call temp$023, $exception := int$java.lang.Object$hashCode$41(o22);
+    assert { :sourceloc "/Users/schaef/git/jar2bpl/jar2bpl_test/regression/true_positives/tp01/InfeasibleCode01.java",35,4,35,23 } true;
+    $return := temp$023;
     return;
-  block4:
-    assert { :sourceloc "/Users/schaef/git/jar2bpl/jar2bpl_test/regression/corner_cases/cc01/CornerCases01.java",18,4,18,10 } true;
-    assert { :sourceloc "/Users/schaef/git/jar2bpl/jar2bpl_test/regression/corner_cases/cc01/CornerCases01.java",19,15,19,22 } true;
-    if (notEqual3 == 0) {
-        assert { :sourceloc "/Users/schaef/git/jar2bpl/jar2bpl_test/regression/corner_cases/cc01/CornerCases01.java",19,15,19,22 } true;
-        goto block7;
-    }
-    assert { :sourceloc "/Users/schaef/git/jar2bpl/jar2bpl_test/regression/corner_cases/cc01/CornerCases01.java",19,15,19,22 } true;
-    goto block8;
   block7:
-    assert { :sourceloc "/Users/schaef/git/jar2bpl/jar2bpl_test/regression/corner_cases/cc01/CornerCases01.java",19,15,19,22 } true;
-    assert { :sourceloc "/Users/schaef/git/jar2bpl/jar2bpl_test/regression/corner_cases/cc01/CornerCases01.java",19,27,19,41 } true;
-    if (truthValue2 == 0) {
-        assert { :sourceloc "/Users/schaef/git/jar2bpl/jar2bpl_test/regression/corner_cases/cc01/CornerCases01.java",19,27,19,41 } true;
+    assert { :sourceloc "/Users/schaef/git/jar2bpl/jar2bpl_test/regression/true_positives/tp01/InfeasibleCode01.java",37,3,37,55 } true;
+    temp$124 := java.io.PrintStream$java.lang.System$err237;
+    assert { :sourceloc "/Users/schaef/git/jar2bpl/jar2bpl_test/regression/true_positives/tp01/InfeasibleCode01.java",37,3,37,55 } true;
+    call $fakelocal_0 := $new(java.lang.StringBuffer);
+    temp$225 := $fakelocal_0;
+    assert { :sourceloc "/Users/schaef/git/jar2bpl/jar2bpl_test/regression/true_positives/tp01/InfeasibleCode01.java",37,22,37,53 } true;
+    call $exception := void$java.lang.StringBuffer$$la$init$ra$$685(temp$225);
+    assert { :sourceloc "/Users/schaef/git/jar2bpl/jar2bpl_test/regression/true_positives/tp01/InfeasibleCode01.java",37,22,37,53 } true;
+    assert { :sourceloc "/Users/schaef/git/jar2bpl/jar2bpl_test/regression/true_positives/tp01/InfeasibleCode01.java",37,22,37,53 } o22 != $null;
+    call temp$326, $exception := java.lang.String$java.lang.Object$toString$44(o22);
+    assert { :sourceloc "/Users/schaef/git/jar2bpl/jar2bpl_test/regression/true_positives/tp01/InfeasibleCode01.java",37,22,37,53 } true;
+    call $fakelocal_1, $exception := java.lang.StringBuffer$java.lang.StringBuffer$append$701(temp$225, temp$326);
+    assert { :sourceloc "/Users/schaef/git/jar2bpl/jar2bpl_test/regression/true_positives/tp01/InfeasibleCode01.java",37,22,37,53 } true;
+    call $fakelocal_2, $exception := java.lang.StringBuffer$java.lang.StringBuffer$append$701(temp$225, $StringConst0);
+    assert { :sourceloc "/Users/schaef/git/jar2bpl/jar2bpl_test/regression/true_positives/tp01/InfeasibleCode01.java",37,22,37,53 } true;
+    call temp$427, $exception := java.lang.String$java.lang.StringBuffer$toString$738(temp$225);
+    assert { :sourceloc "/Users/schaef/git/jar2bpl/jar2bpl_test/regression/true_positives/tp01/InfeasibleCode01.java",37,22,37,53 } true;
+    assert { :sourceloc "/Users/schaef/git/jar2bpl/jar2bpl_test/regression/true_positives/tp01/InfeasibleCode01.java",37,22,37,53 } temp$124 != $null;
+    call $exception := void$java.io.PrintStream$println$217(temp$124, temp$427);
+    assert { :sourceloc "/Users/schaef/git/jar2bpl/jar2bpl_test/regression/true_positives/tp01/InfeasibleCode01.java",37,22,37,53 } true;
+    temp$528 := 2;
+    assert { :sourceloc "/Users/schaef/git/jar2bpl/jar2bpl_test/regression/true_positives/tp01/InfeasibleCode01.java",38,3,38,11 } true;
+    $return := temp$528;
+    return;
+}
+
+
+implementation void$InfeasibleCode01$infeasible2$1892($this:ref, $in_parameter__0:ref) returns ($exception:ref){
+    
+var i31 : int;    
+var temp$234 : int;    
+var temp$436 : int;    
+var temp$335 : int;    
+var arr30 : ref;    
+var temp$133 : ref;    
+var this29 : ref;    
+var temp$032 : int;
+    assume { :sourceloc "/Users/schaef/git/jar2bpl/jar2bpl_test/regression/true_positives/tp01/InfeasibleCode01.java",-1,-1,-1,-1 } $this != $null;
+    assert { :sourceloc "/Users/schaef/git/jar2bpl/jar2bpl_test/regression/true_positives/tp01/InfeasibleCode01.java",41,2,45,2 } true;
+    this29 := $this;
+    assert { :sourceloc "/Users/schaef/git/jar2bpl/jar2bpl_test/regression/true_positives/tp01/InfeasibleCode01.java",41,26,41,35 } true;
+    arr30 := $in_parameter__0;
+    assert { :sourceloc "/Users/schaef/git/jar2bpl/jar2bpl_test/regression/true_positives/tp01/InfeasibleCode01.java",42,8,42,14 } true;
+    i31 := 0;
+  block8:
+    assert { :sourceloc "/Users/schaef/git/jar2bpl/jar2bpl_test/regression/true_positives/tp01/InfeasibleCode01.java",42,17,42,29 } true;
+    assert { :sourceloc "/Users/schaef/git/jar2bpl/jar2bpl_test/regression/true_positives/tp01/InfeasibleCode01.java",42,17,42,29 } arr30 != $null;
+    temp$032 := $arrSizeHeap[arr30];
+    assert { :sourceloc "/Users/schaef/git/jar2bpl/jar2bpl_test/regression/true_positives/tp01/InfeasibleCode01.java",42,17,42,29 } true;
+    if (i31 <= temp$032) {
+        assert { :sourceloc "/Users/schaef/git/jar2bpl/jar2bpl_test/regression/true_positives/tp01/InfeasibleCode01.java",43,4,43,12 } { :comment "thenblock" } true;
         goto block9;
     }
-    assert { :sourceloc "/Users/schaef/git/jar2bpl/jar2bpl_test/regression/corner_cases/cc01/CornerCases01.java",19,27,19,41 } true;
-    goto block8;
-    assert { :sourceloc "/Users/schaef/git/jar2bpl/jar2bpl_test/regression/corner_cases/cc01/CornerCases01.java",19,27,19,41 } true;
-    goto block9;
+    assert { :sourceloc "/Users/schaef/git/jar2bpl/jar2bpl_test/regression/true_positives/tp01/InfeasibleCode01.java",43,4,43,12 } { :comment "elseblock" } true;
+    assert { :sourceloc "/Users/schaef/git/jar2bpl/jar2bpl_test/regression/true_positives/tp01/InfeasibleCode01.java",42,17,42,29 } true;
+    goto block10;
   block9:
-    assert { :sourceloc "/Users/schaef/git/jar2bpl/jar2bpl_test/regression/corner_cases/cc01/CornerCases01.java",19,27,19,41 } true;
-    assert { :sourceloc "/Users/schaef/git/jar2bpl/jar2bpl_test/regression/corner_cases/cc01/CornerCases01.java",20,4,20,10 } true;
-    return;
-  block8:
-    assert { :sourceloc "/Users/schaef/git/jar2bpl/jar2bpl_test/regression/corner_cases/cc01/CornerCases01.java",20,4,20,10 } true;
-    assert { :sourceloc "/Users/schaef/git/jar2bpl/jar2bpl_test/regression/corner_cases/cc01/CornerCases01.java",21,15,21,22 } true;
-    if (notEqual3 == 0) {
-        assert { :sourceloc "/Users/schaef/git/jar2bpl/jar2bpl_test/regression/corner_cases/cc01/CornerCases01.java",21,15,21,22 } true;
-        goto block10;
-    }
-    assert { :sourceloc "/Users/schaef/git/jar2bpl/jar2bpl_test/regression/corner_cases/cc01/CornerCases01.java",21,15,21,22 } true;
-    goto block11;
+    assert { :sourceloc "/Users/schaef/git/jar2bpl/jar2bpl_test/regression/true_positives/tp01/InfeasibleCode01.java",43,4,43,12 } true;
+    temp$133 := arr30;
+    assert { :sourceloc "/Users/schaef/git/jar2bpl/jar2bpl_test/regression/true_positives/tp01/InfeasibleCode01.java",43,4,43,12 } true;
+    temp$234 := i31;
+    assert { :sourceloc "/Users/schaef/git/jar2bpl/jar2bpl_test/regression/true_positives/tp01/InfeasibleCode01.java",43,7,43,9 } true;
+    assert { :sourceloc "/Users/schaef/git/jar2bpl/jar2bpl_test/regression/true_positives/tp01/InfeasibleCode01.java",43,7,43,9 } temp$234 < $arrSizeHeap[temp$133] && temp$234 >= 0;
+    $intArrHeap := $intArrHeap[temp$133 := $intArrHeap[temp$133][temp$234 := i31]];
+    assert { :sourceloc "/Users/schaef/git/jar2bpl/jar2bpl_test/regression/true_positives/tp01/InfeasibleCode01.java",42,31,42,33 } true;
+    temp$335 := i31;
+    assert { :sourceloc "/Users/schaef/git/jar2bpl/jar2bpl_test/regression/true_positives/tp01/InfeasibleCode01.java",42,31,42,31 } true;
+    temp$436 := temp$335 + 1;
+    assert { :sourceloc "/Users/schaef/git/jar2bpl/jar2bpl_test/regression/true_positives/tp01/InfeasibleCode01.java",42,31,42,31 } true;
+    i31 := temp$436;
+    assert { :sourceloc "/Users/schaef/git/jar2bpl/jar2bpl_test/regression/true_positives/tp01/InfeasibleCode01.java",42,3,44,3 } true;
+    goto block8;
   block10:
-    assert { :sourceloc "/Users/schaef/git/jar2bpl/jar2bpl_test/regression/corner_cases/cc01/CornerCases01.java",21,15,21,22 } true;
-    assert { :sourceloc "/Users/schaef/git/jar2bpl/jar2bpl_test/regression/corner_cases/cc01/CornerCases01.java",21,27,21,41 } true;
-    if (truthValue2 == 1) {
-        assert { :sourceloc "/Users/schaef/git/jar2bpl/jar2bpl_test/regression/corner_cases/cc01/CornerCases01.java",21,27,21,41 } true;
-        goto block12;
-    }
-    assert { :sourceloc "/Users/schaef/git/jar2bpl/jar2bpl_test/regression/corner_cases/cc01/CornerCases01.java",21,27,21,41 } true;
-    goto block11;
-    assert { :sourceloc "/Users/schaef/git/jar2bpl/jar2bpl_test/regression/corner_cases/cc01/CornerCases01.java",21,27,21,41 } true;
-    goto block12;
-  block12:
-    assert { :sourceloc "/Users/schaef/git/jar2bpl/jar2bpl_test/regression/corner_cases/cc01/CornerCases01.java",21,27,21,41 } true;
-    assert { :sourceloc "/Users/schaef/git/jar2bpl/jar2bpl_test/regression/corner_cases/cc01/CornerCases01.java",22,4,22,10 } true;
-    return;
-  block11:
-    assert { :sourceloc "/Users/schaef/git/jar2bpl/jar2bpl_test/regression/corner_cases/cc01/CornerCases01.java",22,4,22,10 } true;
-    assert { :sourceloc "/Users/schaef/git/jar2bpl/jar2bpl_test/regression/corner_cases/cc01/CornerCases01.java",24,4,24,32 } true;
-    call $fakelocal_0 := $new(java.lang.RuntimeException);
-    temp$04 := $fakelocal_0;
-    assert { :sourceloc "/Users/schaef/git/jar2bpl/jar2bpl_test/regression/corner_cases/cc01/CornerCases01.java",24,10,24,31 } true;
-    call $exception := void$java.lang.RuntimeException$$la$init$ra$$922(temp$04);
-    assert { :sourceloc "/Users/schaef/git/jar2bpl/jar2bpl_test/regression/corner_cases/cc01/CornerCases01.java",24,10,24,31 } true;
-    $exception := temp$04;
-    return;
-    assert { :sourceloc "/Users/schaef/git/jar2bpl/jar2bpl_test/regression/corner_cases/cc01/CornerCases01.java",24,10,24,31 } true;
+    assert { :sourceloc "/Users/schaef/git/jar2bpl/jar2bpl_test/regression/true_positives/tp01/InfeasibleCode01.java",42,3,44,3 } true;
     return;
 }
 
 
-implementation int$CornerCases01$decisions$1890($this:ref, $in_parameter__0:int, $in_parameter__1:int) returns ($return:int, $exception:ref){
+implementation void$InfeasibleCode01$infeasible3$1893($this:ref, $in_parameter__0:int, $in_parameter__1:int) returns ($exception:ref){
     
-var uppercheck7 : int;    
-var temp$311 : int;    
-var this5 : ref;    
-var temp$19 : int;    
-var temp$08 : int;    
-var temp$210 : int;    
-var lowercheck6 : int;
-    assume { :sourceloc "/Users/schaef/git/jar2bpl/jar2bpl_test/regression/corner_cases/cc01/CornerCases01.java",-1,-1,-1,-1 } $this != $null;
-    assert { :sourceloc "/Users/schaef/git/jar2bpl/jar2bpl_test/regression/corner_cases/cc01/CornerCases01.java",27,2,32,2 } true;
-    this5 := $this;
-    assert { :sourceloc "/Users/schaef/git/jar2bpl/jar2bpl_test/regression/corner_cases/cc01/CornerCases01.java",27,23,27,40 } true;
-    lowercheck6 := $in_parameter__0;
-    assert { :sourceloc "/Users/schaef/git/jar2bpl/jar2bpl_test/regression/corner_cases/cc01/CornerCases01.java",27,43,27,60 } true;
-    uppercheck7 := $in_parameter__1;
-    assert { :sourceloc "/Users/schaef/git/jar2bpl/jar2bpl_test/regression/corner_cases/cc01/CornerCases01.java",28,13,28,22 } true;
-    if (lowercheck6 == 0) {
-        assert { :sourceloc "/Users/schaef/git/jar2bpl/jar2bpl_test/regression/corner_cases/cc01/CornerCases01.java",28,39,28,47 } true;
+var temp$545 : int;    
+var temp$444 : int;    
+var temp$343 : int;    
+var temp$141 : int;    
+var a38 : int;    
+var temp$040 : int;    
+var b39 : int;    
+var temp$242 : int;    
+var this37 : ref;
+    assume { :sourceloc "/Users/schaef/git/jar2bpl/jar2bpl_test/regression/true_positives/tp01/InfeasibleCode01.java",-1,-1,-1,-1 } $this != $null;
+    assert { :sourceloc "/Users/schaef/git/jar2bpl/jar2bpl_test/regression/true_positives/tp01/InfeasibleCode01.java",47,2,52,2 } true;
+    this37 := $this;
+    assert { :sourceloc "/Users/schaef/git/jar2bpl/jar2bpl_test/regression/true_positives/tp01/InfeasibleCode01.java",47,26,47,30 } true;
+    a38 := $in_parameter__0;
+    assert { :sourceloc "/Users/schaef/git/jar2bpl/jar2bpl_test/regression/true_positives/tp01/InfeasibleCode01.java",47,33,47,37 } true;
+    b39 := $in_parameter__1;
+    assert { :sourceloc "/Users/schaef/git/jar2bpl/jar2bpl_test/regression/true_positives/tp01/InfeasibleCode01.java",48,3,48,3 } true;
+    temp$040 := 1;
+    assert { :sourceloc "/Users/schaef/git/jar2bpl/jar2bpl_test/regression/true_positives/tp01/InfeasibleCode01.java",48,3,48,3 } true;
+    b39 := temp$040;
+    assert { :sourceloc "/Users/schaef/git/jar2bpl/jar2bpl_test/regression/true_positives/tp01/InfeasibleCode01.java",49,7,49,9 } true;
+    if (a38 > 0) {
+        assert { :sourceloc "/Users/schaef/git/jar2bpl/jar2bpl_test/regression/true_positives/tp01/InfeasibleCode01.java",49,12,49,15 } { :comment "thenblock" } true;
+        goto block11;
+    }
+    assert { :sourceloc "/Users/schaef/git/jar2bpl/jar2bpl_test/regression/true_positives/tp01/InfeasibleCode01.java",49,12,49,15 } { :comment "elseblock" } true;
+    assert { :sourceloc "/Users/schaef/git/jar2bpl/jar2bpl_test/regression/true_positives/tp01/InfeasibleCode01.java",49,7,49,9 } true;
+    goto block12;
+  block11:
+    assert { :sourceloc "/Users/schaef/git/jar2bpl/jar2bpl_test/regression/true_positives/tp01/InfeasibleCode01.java",49,12,49,15 } true;
+    temp$141 := b39;
+    assert { :sourceloc "/Users/schaef/git/jar2bpl/jar2bpl_test/regression/true_positives/tp01/InfeasibleCode01.java",49,12,49,12 } true;
+    temp$242 := temp$141 + -1;
+    assert { :sourceloc "/Users/schaef/git/jar2bpl/jar2bpl_test/regression/true_positives/tp01/InfeasibleCode01.java",49,12,49,12 } true;
+    b39 := temp$242;
+  block12:
+    assert { :sourceloc "/Users/schaef/git/jar2bpl/jar2bpl_test/regression/true_positives/tp01/InfeasibleCode01.java",50,3,50,8 } true;
+    assert { :sourceloc "/Users/schaef/git/jar2bpl/jar2bpl_test/regression/true_positives/tp01/InfeasibleCode01.java",50,3,50,8 } b39 != 0;
+    temp$343 := 1 div b39;
+    assert { :sourceloc "/Users/schaef/git/jar2bpl/jar2bpl_test/regression/true_positives/tp01/InfeasibleCode01.java",50,3,50,3 } true;
+    b39 := temp$343;
+    assert { :sourceloc "/Users/schaef/git/jar2bpl/jar2bpl_test/regression/true_positives/tp01/InfeasibleCode01.java",51,7,51,10 } true;
+    if (a38 <= 0) {
+        assert { :sourceloc "/Users/schaef/git/jar2bpl/jar2bpl_test/regression/true_positives/tp01/InfeasibleCode01.java",51,13,51,22 } { :comment "thenblock" } true;
         goto block13;
     }
-    assert { :sourceloc "/Users/schaef/git/jar2bpl/jar2bpl_test/regression/corner_cases/cc01/CornerCases01.java",28,13,28,22 } true;
+    assert { :sourceloc "/Users/schaef/git/jar2bpl/jar2bpl_test/regression/true_positives/tp01/InfeasibleCode01.java",51,13,51,22 } { :comment "elseblock" } true;
+    assert { :sourceloc "/Users/schaef/git/jar2bpl/jar2bpl_test/regression/true_positives/tp01/InfeasibleCode01.java",51,7,51,10 } true;
     goto block14;
-  block14:
-    assert { :sourceloc "/Users/schaef/git/jar2bpl/jar2bpl_test/regression/corner_cases/cc01/CornerCases01.java",28,13,28,22 } true;
-    assert { :sourceloc "/Users/schaef/git/jar2bpl/jar2bpl_test/regression/corner_cases/cc01/CornerCases01.java",28,27,28,36 } true;
-    if (uppercheck7 == 0) {
-        assert { :sourceloc "/Users/schaef/git/jar2bpl/jar2bpl_test/regression/corner_cases/cc01/CornerCases01.java",28,39,28,47 } true;
-        goto block13;
-    }
-    assert { :sourceloc "/Users/schaef/git/jar2bpl/jar2bpl_test/regression/corner_cases/cc01/CornerCases01.java",28,27,28,36 } true;
-    goto block15;
-    assert { :sourceloc "/Users/schaef/git/jar2bpl/jar2bpl_test/regression/corner_cases/cc01/CornerCases01.java",28,27,28,36 } true;
-    goto block15;
-  block15:
-    assert { :sourceloc "/Users/schaef/git/jar2bpl/jar2bpl_test/regression/corner_cases/cc01/CornerCases01.java",28,27,28,36 } true;
-    assert { :sourceloc "/Users/schaef/git/jar2bpl/jar2bpl_test/regression/corner_cases/cc01/CornerCases01.java",28,27,28,36 } true;
-    temp$08 := 0;
-    assert { :sourceloc "/Users/schaef/git/jar2bpl/jar2bpl_test/regression/corner_cases/cc01/CornerCases01.java",28,39,28,47 } true;
-    $return := temp$08;
-    return;
   block13:
-    assert { :sourceloc "/Users/schaef/git/jar2bpl/jar2bpl_test/regression/corner_cases/cc01/CornerCases01.java",28,39,28,47 } true;
-    assert { :sourceloc "/Users/schaef/git/jar2bpl/jar2bpl_test/regression/corner_cases/cc01/CornerCases01.java",29,18,29,27 } true;
-    if (lowercheck6 == 0) {
-        assert { :sourceloc "/Users/schaef/git/jar2bpl/jar2bpl_test/regression/corner_cases/cc01/CornerCases01.java",29,45,29,53 } true;
-        goto block16;
+    assert { :sourceloc "/Users/schaef/git/jar2bpl/jar2bpl_test/regression/true_positives/tp01/InfeasibleCode01.java",51,13,51,22 } true;
+    temp$444 := 1 - b39;
+    assert { :sourceloc "/Users/schaef/git/jar2bpl/jar2bpl_test/regression/true_positives/tp01/InfeasibleCode01.java",51,13,51,22 } true;
+    assert { :sourceloc "/Users/schaef/git/jar2bpl/jar2bpl_test/regression/true_positives/tp01/InfeasibleCode01.java",51,13,51,22 } temp$444 != 0;
+    temp$545 := 1 div temp$444;
+  block14:
+    assert { :sourceloc "/Users/schaef/git/jar2bpl/jar2bpl_test/regression/true_positives/tp01/InfeasibleCode01.java",51,13,51,13 } true;
+    return;
+}
+
+
+implementation boolean$InfeasibleCode01$infeasible4$1894($this:ref, $in_parameter__0:ref) returns ($return:int, $exception:ref){
+    
+var temp$048 : ref;    
+var o47 : ref;    
+var temp$250 : int;    
+var this46 : ref;    
+var temp$149 : ref;    
+var temp$351 : int;
+    assume { :sourceloc "/Users/schaef/git/jar2bpl/jar2bpl_test/regression/true_positives/tp01/InfeasibleCode01.java",-1,-1,-1,-1 } $this != $null;
+    assume $heap[$in_parameter__0,$type] <: java.lang.Object;
+    assert { :sourceloc "/Users/schaef/git/jar2bpl/jar2bpl_test/regression/true_positives/tp01/InfeasibleCode01.java",54,2,60,2 } true;
+    this46 := $this;
+    assert { :sourceloc "/Users/schaef/git/jar2bpl/jar2bpl_test/regression/true_positives/tp01/InfeasibleCode01.java",54,29,54,36 } true;
+    o47 := $in_parameter__0;
+    assert { :sourceloc "/Users/schaef/git/jar2bpl/jar2bpl_test/regression/true_positives/tp01/InfeasibleCode01.java",55,3,55,35 } true;
+    temp$048 := java.io.PrintStream$java.lang.System$err237;
+    assert { :sourceloc "/Users/schaef/git/jar2bpl/jar2bpl_test/regression/true_positives/tp01/InfeasibleCode01.java",55,3,55,35 } true;
+    assert { :sourceloc "/Users/schaef/git/jar2bpl/jar2bpl_test/regression/true_positives/tp01/InfeasibleCode01.java",55,3,55,35 } o47 != $null;
+    call temp$149, $exception := java.lang.String$java.lang.Object$toString$44(o47);
+    assert { :sourceloc "/Users/schaef/git/jar2bpl/jar2bpl_test/regression/true_positives/tp01/InfeasibleCode01.java",55,3,55,35 } true;
+    assert { :sourceloc "/Users/schaef/git/jar2bpl/jar2bpl_test/regression/true_positives/tp01/InfeasibleCode01.java",55,3,55,35 } temp$048 != $null;
+    call $exception := void$java.io.PrintStream$println$217(temp$048, temp$149);
+    assert { :sourceloc "/Users/schaef/git/jar2bpl/jar2bpl_test/regression/true_positives/tp01/InfeasibleCode01.java",56,7,56,13 } true;
+    if (o47 == $null) {
+        assert { :sourceloc "/Users/schaef/git/jar2bpl/jar2bpl_test/regression/true_positives/tp01/InfeasibleCode01.java",56,7,56,13 } { :comment "thenblock" } true;
+        goto block15;
     }
-    assert { :sourceloc "/Users/schaef/git/jar2bpl/jar2bpl_test/regression/corner_cases/cc01/CornerCases01.java",29,18,29,27 } true;
-    goto block17;
-  block17:
-    assert { :sourceloc "/Users/schaef/git/jar2bpl/jar2bpl_test/regression/corner_cases/cc01/CornerCases01.java",29,18,29,27 } true;
-    assert { :sourceloc "/Users/schaef/git/jar2bpl/jar2bpl_test/regression/corner_cases/cc01/CornerCases01.java",29,33,29,42 } true;
-    if (uppercheck7 == 0) {
-        assert { :sourceloc "/Users/schaef/git/jar2bpl/jar2bpl_test/regression/corner_cases/cc01/CornerCases01.java",29,33,29,42 } true;
-        goto block18;
-    }
-    assert { :sourceloc "/Users/schaef/git/jar2bpl/jar2bpl_test/regression/corner_cases/cc01/CornerCases01.java",29,33,29,42 } true;
+    assert { :sourceloc "/Users/schaef/git/jar2bpl/jar2bpl_test/regression/true_positives/tp01/InfeasibleCode01.java",56,7,56,13 } { :comment "elseblock" } true;
+    assert { :sourceloc "/Users/schaef/git/jar2bpl/jar2bpl_test/regression/true_positives/tp01/InfeasibleCode01.java",56,7,56,13 } true;
     goto block16;
-    assert { :sourceloc "/Users/schaef/git/jar2bpl/jar2bpl_test/regression/corner_cases/cc01/CornerCases01.java",29,33,29,42 } true;
-    goto block18;
-  block18:
-    assert { :sourceloc "/Users/schaef/git/jar2bpl/jar2bpl_test/regression/corner_cases/cc01/CornerCases01.java",29,33,29,42 } true;
-    assert { :sourceloc "/Users/schaef/git/jar2bpl/jar2bpl_test/regression/corner_cases/cc01/CornerCases01.java",29,33,29,42 } true;
-    temp$19 := 1;
-    assert { :sourceloc "/Users/schaef/git/jar2bpl/jar2bpl_test/regression/corner_cases/cc01/CornerCases01.java",29,45,29,53 } true;
-    $return := temp$19;
+  block15:
+    assert { :sourceloc "/Users/schaef/git/jar2bpl/jar2bpl_test/regression/true_positives/tp01/InfeasibleCode01.java",56,7,56,13 } true;
+    temp$250 := 0;
+    assert { :sourceloc "/Users/schaef/git/jar2bpl/jar2bpl_test/regression/true_positives/tp01/InfeasibleCode01.java",57,4,57,16 } true;
+    $return := temp$250;
     return;
   block16:
-    assert { :sourceloc "/Users/schaef/git/jar2bpl/jar2bpl_test/regression/corner_cases/cc01/CornerCases01.java",29,45,29,53 } true;
-    assert { :sourceloc "/Users/schaef/git/jar2bpl/jar2bpl_test/regression/corner_cases/cc01/CornerCases01.java",30,19,30,28 } true;
-    if (lowercheck6 == 0) {
-        assert { :sourceloc "/Users/schaef/git/jar2bpl/jar2bpl_test/regression/corner_cases/cc01/CornerCases01.java",30,19,30,28 } true;
-        goto block19;
+    assert { :sourceloc "/Users/schaef/git/jar2bpl/jar2bpl_test/regression/true_positives/tp01/InfeasibleCode01.java",57,4,57,16 } true;
+    temp$351 := 1;
+    assert { :sourceloc "/Users/schaef/git/jar2bpl/jar2bpl_test/regression/true_positives/tp01/InfeasibleCode01.java",59,3,59,14 } true;
+    $return := temp$351;
+    return;
+}
+
+
+implementation void$InfeasibleCode01$infeasible5$1895($this:ref) returns ($exception:ref){
+    
+var temp$155 : ref;    
+var test53 : ref;    
+var temp$054 : int;    
+var $fakelocal_0 : ref;    
+var this52 : ref;
+    assume { :sourceloc "/Users/schaef/git/jar2bpl/jar2bpl_test/regression/true_positives/tp01/InfeasibleCode01.java",-1,-1,-1,-1 } $this != $null;
+    assert { :sourceloc "/Users/schaef/git/jar2bpl/jar2bpl_test/regression/true_positives/tp01/InfeasibleCode01.java",62,2,67,2 } true;
+    this52 := $this;
+    assert { :sourceloc "/Users/schaef/git/jar2bpl/jar2bpl_test/regression/true_positives/tp01/InfeasibleCode01.java",63,3,63,25 } true;
+    call $fakelocal_0 := $new(java.lang.String);
+    $stringSizeHeap := $stringSizeHeap[$fakelocal_0 := 8];
+    test53 := $fakelocal_0;
+    assert { :sourceloc "/Users/schaef/git/jar2bpl/jar2bpl_test/regression/true_positives/tp01/InfeasibleCode01.java",64,7,64,22 } true;
+    temp$054 := $stringSizeHeap[test53];
+    assert { :sourceloc "/Users/schaef/git/jar2bpl/jar2bpl_test/regression/true_positives/tp01/InfeasibleCode01.java",64,7,64,22 } true;
+    if (temp$054 == 3) {
+        assert { :sourceloc "/Users/schaef/git/jar2bpl/jar2bpl_test/regression/true_positives/tp01/InfeasibleCode01.java",65,4,65,37 } { :comment "thenblock" } true;
+        goto block17;
     }
-    assert { :sourceloc "/Users/schaef/git/jar2bpl/jar2bpl_test/regression/corner_cases/cc01/CornerCases01.java",30,19,30,28 } true;
-    goto block20;
+    assert { :sourceloc "/Users/schaef/git/jar2bpl/jar2bpl_test/regression/true_positives/tp01/InfeasibleCode01.java",65,4,65,37 } { :comment "elseblock" } true;
+    assert { :sourceloc "/Users/schaef/git/jar2bpl/jar2bpl_test/regression/true_positives/tp01/InfeasibleCode01.java",64,7,64,22 } true;
+    goto block18;
+  block17:
+    assert { :sourceloc "/Users/schaef/git/jar2bpl/jar2bpl_test/regression/true_positives/tp01/InfeasibleCode01.java",65,4,65,37 } true;
+    temp$155 := java.io.PrintStream$java.lang.System$err237;
+    assert { :sourceloc "/Users/schaef/git/jar2bpl/jar2bpl_test/regression/true_positives/tp01/InfeasibleCode01.java",65,4,65,37 } true;
+    assert { :sourceloc "/Users/schaef/git/jar2bpl/jar2bpl_test/regression/true_positives/tp01/InfeasibleCode01.java",65,4,65,37 } temp$155 != $null;
+    call $exception := void$java.io.PrintStream$println$217(temp$155, $StringConst1);
+  block18:
+    assert { :sourceloc "/Users/schaef/git/jar2bpl/jar2bpl_test/regression/true_positives/tp01/InfeasibleCode01.java",65,4,65,37 } true;
+    return;
+}
+
+
+implementation int$InfeasibleCode01$infeasible6$1896($this:ref, $in_parameter__0:ref) returns ($return:int, $exception:ref){
+    
+var temp$563 : int;    
+var arr57 : ref;    
+var temp$462 : int;    
+var temp$159 : int;    
+var this56 : ref;    
+var temp$058 : ref;    
+var temp$664 : int;    
+var temp$260 : int;    
+var temp$361 : ref;
+    assume { :sourceloc "/Users/schaef/git/jar2bpl/jar2bpl_test/regression/true_positives/tp01/InfeasibleCode01.java",-1,-1,-1,-1 } $this != $null;
+    assert { :sourceloc "/Users/schaef/git/jar2bpl/jar2bpl_test/regression/true_positives/tp01/InfeasibleCode01.java",69,2,71,2 } true;
+    this56 := $this;
+    assert { :sourceloc "/Users/schaef/git/jar2bpl/jar2bpl_test/regression/true_positives/tp01/InfeasibleCode01.java",69,25,69,33 } true;
+    arr57 := $in_parameter__0;
+    assert { :sourceloc "/Users/schaef/git/jar2bpl/jar2bpl_test/regression/true_positives/tp01/InfeasibleCode01.java",69,25,69,33 } true;
+    temp$058 := arr57;
+    assert { :sourceloc "/Users/schaef/git/jar2bpl/jar2bpl_test/regression/true_positives/tp01/InfeasibleCode01.java",69,25,69,33 } true;
+    temp$159 := -1;
+    assert { :sourceloc "/Users/schaef/git/jar2bpl/jar2bpl_test/regression/true_positives/tp01/InfeasibleCode01.java",69,25,69,33 } true;
+    assert { :sourceloc "/Users/schaef/git/jar2bpl/jar2bpl_test/regression/true_positives/tp01/InfeasibleCode01.java",69,25,69,33 } temp$159 < $arrSizeHeap[temp$058] && temp$159 >= 0;
+    temp$260 := $intArrHeap[temp$058][temp$159];
+    assert { :sourceloc "/Users/schaef/git/jar2bpl/jar2bpl_test/regression/true_positives/tp01/InfeasibleCode01.java",69,25,69,33 } true;
+    temp$361 := arr57;
+    assert { :sourceloc "/Users/schaef/git/jar2bpl/jar2bpl_test/regression/true_positives/tp01/InfeasibleCode01.java",69,25,69,33 } true;
+    assert { :sourceloc "/Users/schaef/git/jar2bpl/jar2bpl_test/regression/true_positives/tp01/InfeasibleCode01.java",69,25,69,33 } arr57 != $null;
+    temp$462 := $arrSizeHeap[arr57];
+    assert { :sourceloc "/Users/schaef/git/jar2bpl/jar2bpl_test/regression/true_positives/tp01/InfeasibleCode01.java",69,25,69,33 } true;
+    assert { :sourceloc "/Users/schaef/git/jar2bpl/jar2bpl_test/regression/true_positives/tp01/InfeasibleCode01.java",69,25,69,33 } temp$462 < $arrSizeHeap[temp$361] && temp$462 >= 0;
+    temp$563 := $intArrHeap[temp$361][temp$462];
+    assert { :sourceloc "/Users/schaef/git/jar2bpl/jar2bpl_test/regression/true_positives/tp01/InfeasibleCode01.java",69,25,69,33 } true;
+    temp$664 := temp$260 + temp$563;
+    assert { :sourceloc "/Users/schaef/git/jar2bpl/jar2bpl_test/regression/true_positives/tp01/InfeasibleCode01.java",70,3,70,35 } true;
+    $return := temp$664;
+    return;
+}
+
+
+implementation void$InfeasibleCode01$infeasible07$1897($this:ref, $in_parameter__0:ref) returns ($exception:ref){
+    
+var temp$373 : int;    
+var end68 : int;    
+var temp$070 : int;    
+var temp$575 : int;    
+var temp$777 : int;    
+var temp$676 : int;    
+var repos67 : int;    
+var j69 : int;    
+var temp$878 : int;    
+var temp$272 : ref;    
+var this65 : ref;    
+var temp66 : ref;    
+var temp$171 : int;    
+var temp$474 : int;
+    assume { :sourceloc "/Users/schaef/git/jar2bpl/jar2bpl_test/regression/true_positives/tp01/InfeasibleCode01.java",-1,-1,-1,-1 } $this != $null;
+    assert { :sourceloc "/Users/schaef/git/jar2bpl/jar2bpl_test/regression/true_positives/tp01/InfeasibleCode01.java",73,2,86,2 } true;
+    this65 := $this;
+    assert { :sourceloc "/Users/schaef/git/jar2bpl/jar2bpl_test/regression/true_positives/tp01/InfeasibleCode01.java",73,27,73,37 } true;
+    temp66 := $in_parameter__0;
+    assert { :sourceloc "/Users/schaef/git/jar2bpl/jar2bpl_test/regression/true_positives/tp01/InfeasibleCode01.java",74,3,74,17 } true;
+    repos67 := -1;
+    assert { :sourceloc "/Users/schaef/git/jar2bpl/jar2bpl_test/regression/true_positives/tp01/InfeasibleCode01.java",75,3,75,15 } true;
+    end68 := -1;
+    assert { :sourceloc "/Users/schaef/git/jar2bpl/jar2bpl_test/regression/true_positives/tp01/InfeasibleCode01.java",76,3,76,14 } true;
+    j69 := end68;
   block19:
-    assert { :sourceloc "/Users/schaef/git/jar2bpl/jar2bpl_test/regression/corner_cases/cc01/CornerCases01.java",30,19,30,28 } true;
-    assert { :sourceloc "/Users/schaef/git/jar2bpl/jar2bpl_test/regression/corner_cases/cc01/CornerCases01.java",30,33,30,42 } true;
-    if (uppercheck7 == 0) {
-        assert { :sourceloc "/Users/schaef/git/jar2bpl/jar2bpl_test/regression/corner_cases/cc01/CornerCases01.java",30,45,30,53 } true;
+    assert { :sourceloc "/Users/schaef/git/jar2bpl/jar2bpl_test/regression/true_positives/tp01/InfeasibleCode01.java",78,4,78,7 } true;
+    temp$070 := j69;
+    assert { :sourceloc "/Users/schaef/git/jar2bpl/jar2bpl_test/regression/true_positives/tp01/InfeasibleCode01.java",78,4,78,4 } true;
+    temp$171 := temp$070 + 1;
+    assert { :sourceloc "/Users/schaef/git/jar2bpl/jar2bpl_test/regression/true_positives/tp01/InfeasibleCode01.java",78,4,78,4 } true;
+    j69 := temp$171;
+    assert { :sourceloc "/Users/schaef/git/jar2bpl/jar2bpl_test/regression/true_positives/tp01/InfeasibleCode01.java",79,8,79,19 } true;
+    temp$272 := temp66;
+    assert { :sourceloc "/Users/schaef/git/jar2bpl/jar2bpl_test/regression/true_positives/tp01/InfeasibleCode01.java",79,8,79,19 } true;
+    temp$373 := j69;
+    assert { :sourceloc "/Users/schaef/git/jar2bpl/jar2bpl_test/regression/true_positives/tp01/InfeasibleCode01.java",79,8,79,19 } true;
+    assert { :sourceloc "/Users/schaef/git/jar2bpl/jar2bpl_test/regression/true_positives/tp01/InfeasibleCode01.java",79,8,79,19 } temp$373 < $arrSizeHeap[temp$272] && temp$373 >= 0;
+    temp$474 := $intArrHeap[temp$272][temp$373];
+    assert { :sourceloc "/Users/schaef/git/jar2bpl/jar2bpl_test/regression/true_positives/tp01/InfeasibleCode01.java",79,8,79,19 } true;
+    temp$575 := temp$474;
+    assert { :sourceloc "/Users/schaef/git/jar2bpl/jar2bpl_test/regression/true_positives/tp01/InfeasibleCode01.java",79,8,79,19 } true;
+    if (temp$575 == 97) {
+        assert { :sourceloc "/Users/schaef/git/jar2bpl/jar2bpl_test/regression/true_positives/tp01/InfeasibleCode01.java",80,5,80,24 } { :comment "thenblock" } true;
         goto block20;
     }
-    assert { :sourceloc "/Users/schaef/git/jar2bpl/jar2bpl_test/regression/corner_cases/cc01/CornerCases01.java",30,33,30,42 } true;
+    assert { :sourceloc "/Users/schaef/git/jar2bpl/jar2bpl_test/regression/true_positives/tp01/InfeasibleCode01.java",80,5,80,24 } { :comment "elseblock" } true;
+    assert { :sourceloc "/Users/schaef/git/jar2bpl/jar2bpl_test/regression/true_positives/tp01/InfeasibleCode01.java",79,8,79,19 } true;
     goto block21;
-    assert { :sourceloc "/Users/schaef/git/jar2bpl/jar2bpl_test/regression/corner_cases/cc01/CornerCases01.java",30,33,30,42 } true;
-    goto block21;
-  block21:
-    assert { :sourceloc "/Users/schaef/git/jar2bpl/jar2bpl_test/regression/corner_cases/cc01/CornerCases01.java",30,33,30,42 } true;
-    assert { :sourceloc "/Users/schaef/git/jar2bpl/jar2bpl_test/regression/corner_cases/cc01/CornerCases01.java",30,33,30,42 } true;
-    temp$210 := 2;
-    assert { :sourceloc "/Users/schaef/git/jar2bpl/jar2bpl_test/regression/corner_cases/cc01/CornerCases01.java",30,45,30,53 } true;
-    $return := temp$210;
-    return;
   block20:
-    assert { :sourceloc "/Users/schaef/git/jar2bpl/jar2bpl_test/regression/corner_cases/cc01/CornerCases01.java",30,45,30,53 } true;
-    assert { :sourceloc "/Users/schaef/git/jar2bpl/jar2bpl_test/regression/corner_cases/cc01/CornerCases01.java",30,45,30,53 } true;
-    temp$311 := 3;
-    assert { :sourceloc "/Users/schaef/git/jar2bpl/jar2bpl_test/regression/corner_cases/cc01/CornerCases01.java",31,14,31,22 } true;
-    $return := temp$311;
-    return;
-}
-
-
-implementation int$CornerCases01$getNewIndex$1891($this:ref, $in_parameter__0:int, $in_parameter__1:ref, $in_parameter__2:ref, $in_parameter__3:ref, $in_parameter__4:ref) returns ($return:int, $exception:ref){
-    
-var temp$1030 : int;    
-var temp$019 : int;    
-var rand27 : int;    
-var chars15 : ref;    
-var temp$221 : int;    
-var temp$423 : int;    
-var max18 : int;    
-var temp$828 : int;    
-var temp$524 : int;    
-var temp$120 : int;    
-var booleans17 : ref;    
-var temp$625 : int;    
-var index13 : int;    
-var ints14 : ref;    
-var temp$929 : int;    
-var this12 : ref;    
-var temp$1131 : int;    
-var bytes16 : ref;    
-var temp$726 : int;    
-var temp$1232 : int;    
-var temp$322 : int;
-    assume { :sourceloc "/Users/schaef/git/jar2bpl/jar2bpl_test/regression/corner_cases/cc01/CornerCases01.java",-1,-1,-1,-1 } $this != $null;
-    assume $heap[$in_parameter__2,$type] <: java.util.List;
-    assume $heap[$in_parameter__1,$type] <: java.util.List;
-    assume $heap[$in_parameter__4,$type] <: java.util.List;
-    assume $heap[$in_parameter__3,$type] <: java.util.List;
-    assert { :sourceloc "/Users/schaef/git/jar2bpl/jar2bpl_test/regression/corner_cases/cc01/CornerCases01.java",35,2,57,5 } true;
-    this12 := $this;
-    assert { :sourceloc "/Users/schaef/git/jar2bpl/jar2bpl_test/regression/corner_cases/cc01/CornerCases01.java",35,25,35,33 } true;
-    index13 := $in_parameter__0;
-    assert { :sourceloc "/Users/schaef/git/jar2bpl/jar2bpl_test/regression/corner_cases/cc01/CornerCases01.java",35,36,35,52 } true;
-    ints14 := $in_parameter__1;
-    assert { :sourceloc "/Users/schaef/git/jar2bpl/jar2bpl_test/regression/corner_cases/cc01/CornerCases01.java",35,55,35,72 } true;
-    chars15 := $in_parameter__2;
-    assert { :sourceloc "/Users/schaef/git/jar2bpl/jar2bpl_test/regression/corner_cases/cc01/CornerCases01.java",36,4,36,21 } true;
-    bytes16 := $in_parameter__3;
-    assert { :sourceloc "/Users/schaef/git/jar2bpl/jar2bpl_test/regression/corner_cases/cc01/CornerCases01.java",36,24,36,44 } true;
-    booleans17 := $in_parameter__4;
-    assert { :sourceloc "/Users/schaef/git/jar2bpl/jar2bpl_test/regression/corner_cases/cc01/CornerCases01.java",37,7,37,18 } true;
-    max18 := 0;
-    assert { :sourceloc "/Users/schaef/git/jar2bpl/jar2bpl_test/regression/corner_cases/cc01/CornerCases01.java",38,11,38,29 } true;
-    assert { :sourceloc "/Users/schaef/git/jar2bpl/jar2bpl_test/regression/corner_cases/cc01/CornerCases01.java",38,11,38,29 } booleans17 != $null;
-    call temp$019, $exception := int$java.util.List$size$152(booleans17);
-    assert { :sourceloc "/Users/schaef/git/jar2bpl/jar2bpl_test/regression/corner_cases/cc01/CornerCases01.java",38,11,38,29 } true;
-    if (temp$019 > 0) {
-        assert { :sourceloc "/Users/schaef/git/jar2bpl/jar2bpl_test/regression/corner_cases/cc01/CornerCases01.java",38,11,38,29 } true;
+    assert { :sourceloc "/Users/schaef/git/jar2bpl/jar2bpl_test/regression/true_positives/tp01/InfeasibleCode01.java",80,5,80,24 } true;
+    temp$676 := j69 - end68;
+    assert { :sourceloc "/Users/schaef/git/jar2bpl/jar2bpl_test/regression/true_positives/tp01/InfeasibleCode01.java",80,5,80,24 } true;
+    temp$777 := temp$676 - 1;
+    assert { :sourceloc "/Users/schaef/git/jar2bpl/jar2bpl_test/regression/true_positives/tp01/InfeasibleCode01.java",80,5,80,9 } true;
+    repos67 := temp$777;
+  block21:
+    assert { :sourceloc "/Users/schaef/git/jar2bpl/jar2bpl_test/regression/true_positives/tp01/InfeasibleCode01.java",82,12,82,22 } true;
+    if (repos67 == -1) {
+        assert { :sourceloc "/Users/schaef/git/jar2bpl/jar2bpl_test/regression/true_positives/tp01/InfeasibleCode01.java",82,27,82,41 } { :clone } { :comment "thenblock" } true;
         goto block22;
     }
-    assert { :sourceloc "/Users/schaef/git/jar2bpl/jar2bpl_test/regression/corner_cases/cc01/CornerCases01.java",38,11,38,29 } true;
+    assert { :sourceloc "/Users/schaef/git/jar2bpl/jar2bpl_test/regression/true_positives/tp01/InfeasibleCode01.java",82,27,82,41 } { :clone } { :comment "elseblock" } true;
+    assert { :sourceloc "/Users/schaef/git/jar2bpl/jar2bpl_test/regression/true_positives/tp01/InfeasibleCode01.java",82,12,82,22 } true;
     goto block23;
   block22:
-    assert { :sourceloc "/Users/schaef/git/jar2bpl/jar2bpl_test/regression/corner_cases/cc01/CornerCases01.java",38,11,38,29 } true;
-    assert { :sourceloc "/Users/schaef/git/jar2bpl/jar2bpl_test/regression/corner_cases/cc01/CornerCases01.java",38,34,38,43 } true;
-    if (index13 < 63) {
-        assert { :sourceloc "/Users/schaef/git/jar2bpl/jar2bpl_test/regression/corner_cases/cc01/CornerCases01.java",38,34,38,43 } true;
+    assert { :sourceloc "/Users/schaef/git/jar2bpl/jar2bpl_test/regression/true_positives/tp01/InfeasibleCode01.java",82,27,82,41 } true;
+    assert { :sourceloc "/Users/schaef/git/jar2bpl/jar2bpl_test/regression/true_positives/tp01/InfeasibleCode01.java",82,27,82,41 } temp66 != $null;
+    temp$878 := $arrSizeHeap[temp66];
+    assert { :sourceloc "/Users/schaef/git/jar2bpl/jar2bpl_test/regression/true_positives/tp01/InfeasibleCode01.java",82,27,82,41 } true;
+    if (j69 < temp$878) {
+        assert { :sourceloc "/Users/schaef/git/jar2bpl/jar2bpl_test/regression/true_positives/tp01/InfeasibleCode01.java",78,4,78,7 } { :comment "thenblock" } true;
+        goto block19;
+    }
+    assert { :sourceloc "/Users/schaef/git/jar2bpl/jar2bpl_test/regression/true_positives/tp01/InfeasibleCode01.java",78,4,78,7 } { :comment "elseblock" } true;
+    assert { :sourceloc "/Users/schaef/git/jar2bpl/jar2bpl_test/regression/true_positives/tp01/InfeasibleCode01.java",82,27,82,41 } true;
+    goto block23;
+  block23:
+    assert { :sourceloc "/Users/schaef/git/jar2bpl/jar2bpl_test/regression/true_positives/tp01/InfeasibleCode01.java",83,7,83,17 } true;
+    if (repos67 == -1) {
+        assert { :sourceloc "/Users/schaef/git/jar2bpl/jar2bpl_test/regression/true_positives/tp01/InfeasibleCode01.java",84,4,84,8 } { :clone } { :comment "thenblock" } true;
         goto block24;
     }
-    assert { :sourceloc "/Users/schaef/git/jar2bpl/jar2bpl_test/regression/corner_cases/cc01/CornerCases01.java",38,34,38,43 } true;
-    goto block23;
-    assert { :sourceloc "/Users/schaef/git/jar2bpl/jar2bpl_test/regression/corner_cases/cc01/CornerCases01.java",38,34,38,43 } true;
+    assert { :sourceloc "/Users/schaef/git/jar2bpl/jar2bpl_test/regression/true_positives/tp01/InfeasibleCode01.java",84,4,84,8 } { :clone } { :comment "elseblock" } true;
+    assert { :sourceloc "/Users/schaef/git/jar2bpl/jar2bpl_test/regression/true_positives/tp01/InfeasibleCode01.java",83,7,83,17 } true;
     goto block24;
   block24:
-    assert { :sourceloc "/Users/schaef/git/jar2bpl/jar2bpl_test/regression/corner_cases/cc01/CornerCases01.java",38,34,38,43 } true;
-    assert { :sourceloc "/Users/schaef/git/jar2bpl/jar2bpl_test/regression/corner_cases/cc01/CornerCases01.java",39,9,39,11 } true;
-    temp$120 := 64;
-    assert { :sourceloc "/Users/schaef/git/jar2bpl/jar2bpl_test/regression/corner_cases/cc01/CornerCases01.java",39,9,39,11 } true;
-    max18 := temp$120;
-    assert { :sourceloc "/Users/schaef/git/jar2bpl/jar2bpl_test/regression/corner_cases/cc01/CornerCases01.java",38,7,45,17 } true;
-    goto block25;
-  block23:
-    assert { :sourceloc "/Users/schaef/git/jar2bpl/jar2bpl_test/regression/corner_cases/cc01/CornerCases01.java",38,7,45,17 } true;
-    assert { :sourceloc "/Users/schaef/git/jar2bpl/jar2bpl_test/regression/corner_cases/cc01/CornerCases01.java",40,16,40,31 } true;
-    assert { :sourceloc "/Users/schaef/git/jar2bpl/jar2bpl_test/regression/corner_cases/cc01/CornerCases01.java",40,16,40,31 } bytes16 != $null;
-    call temp$221, $exception := int$java.util.List$size$152(bytes16);
-    assert { :sourceloc "/Users/schaef/git/jar2bpl/jar2bpl_test/regression/corner_cases/cc01/CornerCases01.java",40,16,40,31 } true;
-    if (temp$221 > 0) {
-        assert { :sourceloc "/Users/schaef/git/jar2bpl/jar2bpl_test/regression/corner_cases/cc01/CornerCases01.java",40,16,40,31 } true;
-        goto block26;
-    }
-    assert { :sourceloc "/Users/schaef/git/jar2bpl/jar2bpl_test/regression/corner_cases/cc01/CornerCases01.java",40,16,40,31 } true;
-    goto block27;
-  block26:
-    assert { :sourceloc "/Users/schaef/git/jar2bpl/jar2bpl_test/regression/corner_cases/cc01/CornerCases01.java",40,16,40,31 } true;
-    assert { :sourceloc "/Users/schaef/git/jar2bpl/jar2bpl_test/regression/corner_cases/cc01/CornerCases01.java",40,36,40,45 } true;
-    if (index13 < 56) {
-        assert { :sourceloc "/Users/schaef/git/jar2bpl/jar2bpl_test/regression/corner_cases/cc01/CornerCases01.java",40,36,40,45 } true;
-        goto block28;
-    }
-    assert { :sourceloc "/Users/schaef/git/jar2bpl/jar2bpl_test/regression/corner_cases/cc01/CornerCases01.java",40,36,40,45 } true;
-    goto block27;
-    assert { :sourceloc "/Users/schaef/git/jar2bpl/jar2bpl_test/regression/corner_cases/cc01/CornerCases01.java",40,36,40,45 } true;
-    goto block28;
-  block28:
-    assert { :sourceloc "/Users/schaef/git/jar2bpl/jar2bpl_test/regression/corner_cases/cc01/CornerCases01.java",40,36,40,45 } true;
-    assert { :sourceloc "/Users/schaef/git/jar2bpl/jar2bpl_test/regression/corner_cases/cc01/CornerCases01.java",41,9,41,11 } true;
-    temp$322 := 57;
-    assert { :sourceloc "/Users/schaef/git/jar2bpl/jar2bpl_test/regression/corner_cases/cc01/CornerCases01.java",41,9,41,11 } true;
-    max18 := temp$322;
-    assert { :sourceloc "/Users/schaef/git/jar2bpl/jar2bpl_test/regression/corner_cases/cc01/CornerCases01.java",40,12,45,17 } true;
-    goto block29;
-  block27:
-    assert { :sourceloc "/Users/schaef/git/jar2bpl/jar2bpl_test/regression/corner_cases/cc01/CornerCases01.java",40,12,45,17 } true;
-    assert { :sourceloc "/Users/schaef/git/jar2bpl/jar2bpl_test/regression/corner_cases/cc01/CornerCases01.java",42,16,42,31 } true;
-    assert { :sourceloc "/Users/schaef/git/jar2bpl/jar2bpl_test/regression/corner_cases/cc01/CornerCases01.java",42,16,42,31 } chars15 != $null;
-    call temp$423, $exception := int$java.util.List$size$152(chars15);
-    assert { :sourceloc "/Users/schaef/git/jar2bpl/jar2bpl_test/regression/corner_cases/cc01/CornerCases01.java",42,16,42,31 } true;
-    if (temp$423 > 0) {
-        assert { :sourceloc "/Users/schaef/git/jar2bpl/jar2bpl_test/regression/corner_cases/cc01/CornerCases01.java",42,16,42,31 } true;
-        goto block30;
-    }
-    assert { :sourceloc "/Users/schaef/git/jar2bpl/jar2bpl_test/regression/corner_cases/cc01/CornerCases01.java",42,16,42,31 } true;
-    goto block31;
-  block30:
-    assert { :sourceloc "/Users/schaef/git/jar2bpl/jar2bpl_test/regression/corner_cases/cc01/CornerCases01.java",42,16,42,31 } true;
-    assert { :sourceloc "/Users/schaef/git/jar2bpl/jar2bpl_test/regression/corner_cases/cc01/CornerCases01.java",42,36,42,45 } true;
-    if (index13 < 48) {
-        assert { :sourceloc "/Users/schaef/git/jar2bpl/jar2bpl_test/regression/corner_cases/cc01/CornerCases01.java",42,36,42,45 } true;
-        goto block32;
-    }
-    assert { :sourceloc "/Users/schaef/git/jar2bpl/jar2bpl_test/regression/corner_cases/cc01/CornerCases01.java",42,36,42,45 } true;
-    goto block31;
-    assert { :sourceloc "/Users/schaef/git/jar2bpl/jar2bpl_test/regression/corner_cases/cc01/CornerCases01.java",42,36,42,45 } true;
-    goto block32;
-  block32:
-    assert { :sourceloc "/Users/schaef/git/jar2bpl/jar2bpl_test/regression/corner_cases/cc01/CornerCases01.java",42,36,42,45 } true;
-    assert { :sourceloc "/Users/schaef/git/jar2bpl/jar2bpl_test/regression/corner_cases/cc01/CornerCases01.java",43,9,43,11 } true;
-    temp$524 := 49;
-    assert { :sourceloc "/Users/schaef/git/jar2bpl/jar2bpl_test/regression/corner_cases/cc01/CornerCases01.java",43,9,43,11 } true;
-    max18 := temp$524;
-    assert { :sourceloc "/Users/schaef/git/jar2bpl/jar2bpl_test/regression/corner_cases/cc01/CornerCases01.java",42,12,45,17 } true;
-    goto block33;
-  block31:
-    assert { :sourceloc "/Users/schaef/git/jar2bpl/jar2bpl_test/regression/corner_cases/cc01/CornerCases01.java",42,12,45,17 } true;
-    assert { :sourceloc "/Users/schaef/git/jar2bpl/jar2bpl_test/regression/corner_cases/cc01/CornerCases01.java",44,16,44,30 } true;
-    assert { :sourceloc "/Users/schaef/git/jar2bpl/jar2bpl_test/regression/corner_cases/cc01/CornerCases01.java",44,16,44,30 } ints14 != $null;
-    call temp$625, $exception := int$java.util.List$size$152(ints14);
-    assert { :sourceloc "/Users/schaef/git/jar2bpl/jar2bpl_test/regression/corner_cases/cc01/CornerCases01.java",44,16,44,30 } true;
-    if (temp$625 > 0) {
-        assert { :sourceloc "/Users/schaef/git/jar2bpl/jar2bpl_test/regression/corner_cases/cc01/CornerCases01.java",44,16,44,30 } true;
-        goto block34;
-    }
-    assert { :sourceloc "/Users/schaef/git/jar2bpl/jar2bpl_test/regression/corner_cases/cc01/CornerCases01.java",44,16,44,30 } true;
-    goto block35;
-  block34:
-    assert { :sourceloc "/Users/schaef/git/jar2bpl/jar2bpl_test/regression/corner_cases/cc01/CornerCases01.java",44,16,44,30 } true;
-    assert { :sourceloc "/Users/schaef/git/jar2bpl/jar2bpl_test/regression/corner_cases/cc01/CornerCases01.java",44,35,44,44 } true;
-    if (index13 < 32) {
-        assert { :sourceloc "/Users/schaef/git/jar2bpl/jar2bpl_test/regression/corner_cases/cc01/CornerCases01.java",44,35,44,44 } true;
-        goto block36;
-    }
-    assert { :sourceloc "/Users/schaef/git/jar2bpl/jar2bpl_test/regression/corner_cases/cc01/CornerCases01.java",44,35,44,44 } true;
-    goto block35;
-    assert { :sourceloc "/Users/schaef/git/jar2bpl/jar2bpl_test/regression/corner_cases/cc01/CornerCases01.java",44,35,44,44 } true;
-    goto block36;
-  block36:
-    assert { :sourceloc "/Users/schaef/git/jar2bpl/jar2bpl_test/regression/corner_cases/cc01/CornerCases01.java",44,35,44,44 } true;
-    assert { :sourceloc "/Users/schaef/git/jar2bpl/jar2bpl_test/regression/corner_cases/cc01/CornerCases01.java",45,9,45,11 } true;
-    temp$726 := 33;
-    assert { :sourceloc "/Users/schaef/git/jar2bpl/jar2bpl_test/regression/corner_cases/cc01/CornerCases01.java",45,9,45,11 } true;
-    max18 := temp$726;
-  block35:
-    assert { :sourceloc "/Users/schaef/git/jar2bpl/jar2bpl_test/regression/corner_cases/cc01/CornerCases01.java",45,9,45,11 } true;
-  block33:
-    assert { :sourceloc "/Users/schaef/git/jar2bpl/jar2bpl_test/regression/corner_cases/cc01/CornerCases01.java",45,9,45,11 } true;
-  block29:
-    assert { :sourceloc "/Users/schaef/git/jar2bpl/jar2bpl_test/regression/corner_cases/cc01/CornerCases01.java",45,9,45,11 } true;
-  block25:
-    assert { :sourceloc "/Users/schaef/git/jar2bpl/jar2bpl_test/regression/corner_cases/cc01/CornerCases01.java",45,9,45,11 } true;
-    assert { :sourceloc "/Users/schaef/git/jar2bpl/jar2bpl_test/regression/corner_cases/cc01/CornerCases01.java",47,11,47,18 } true;
-    if (max18 != 0) {
-        assert { :sourceloc "/Users/schaef/git/jar2bpl/jar2bpl_test/regression/corner_cases/cc01/CornerCases01.java",47,11,47,18 } true;
-        goto block37;
-    }
-    assert { :sourceloc "/Users/schaef/git/jar2bpl/jar2bpl_test/regression/corner_cases/cc01/CornerCases01.java",47,11,47,18 } true;
-    goto block38;
-  block37:
-    assert { :sourceloc "/Users/schaef/git/jar2bpl/jar2bpl_test/regression/corner_cases/cc01/CornerCases01.java",47,11,47,18 } true;
-    assert { :sourceloc "/Users/schaef/git/jar2bpl/jar2bpl_test/regression/corner_cases/cc01/CornerCases01.java",48,20,48,28 } true;
-    call temp$828, $exception := int$CornerCases01$getInt$1892(this12, 4);
-    assert { :sourceloc "/Users/schaef/git/jar2bpl/jar2bpl_test/regression/corner_cases/cc01/CornerCases01.java",48,20,48,28 } true;
-    rand27 := temp$828;
-    assert { :sourceloc "/Users/schaef/git/jar2bpl/jar2bpl_test/regression/corner_cases/cc01/CornerCases01.java",49,9,49,26 } true;
-    temp$929 := max18 - index13;
-    assert { :sourceloc "/Users/schaef/git/jar2bpl/jar2bpl_test/regression/corner_cases/cc01/CornerCases01.java",49,9,49,11 } true;
-    max18 := temp$929;
-    assert { :sourceloc "/Users/schaef/git/jar2bpl/jar2bpl_test/regression/corner_cases/cc01/CornerCases01.java",50,13,50,22 } true;
-    if (max18 > rand27) {
-        assert { :sourceloc "/Users/schaef/git/jar2bpl/jar2bpl_test/regression/corner_cases/cc01/CornerCases01.java",50,13,50,22 } true;
-        goto block39;
-    }
-    assert { :sourceloc "/Users/schaef/git/jar2bpl/jar2bpl_test/regression/corner_cases/cc01/CornerCases01.java",50,13,50,22 } true;
-    goto block40;
-  block39:
-    assert { :sourceloc "/Users/schaef/git/jar2bpl/jar2bpl_test/regression/corner_cases/cc01/CornerCases01.java",50,13,50,22 } true;
-    assert { :sourceloc "/Users/schaef/git/jar2bpl/jar2bpl_test/regression/corner_cases/cc01/CornerCases01.java",51,11,51,13 } true;
-    max18 := rand27;
-    assert { :sourceloc "/Users/schaef/git/jar2bpl/jar2bpl_test/regression/corner_cases/cc01/CornerCases01.java",50,9,53,28 } true;
-    goto block41;
-  block40:
-    assert { :sourceloc "/Users/schaef/git/jar2bpl/jar2bpl_test/regression/corner_cases/cc01/CornerCases01.java",50,9,53,28 } true;
-    assert { :sourceloc "/Users/schaef/git/jar2bpl/jar2bpl_test/regression/corner_cases/cc01/CornerCases01.java",52,18,52,25 } true;
-    if (max18 != 1) {
-        assert { :sourceloc "/Users/schaef/git/jar2bpl/jar2bpl_test/regression/corner_cases/cc01/CornerCases01.java",52,18,52,25 } true;
-        goto block42;
-    }
-    assert { :sourceloc "/Users/schaef/git/jar2bpl/jar2bpl_test/regression/corner_cases/cc01/CornerCases01.java",52,18,52,25 } true;
-    goto block43;
-  block42:
-    assert { :sourceloc "/Users/schaef/git/jar2bpl/jar2bpl_test/regression/corner_cases/cc01/CornerCases01.java",52,18,52,25 } true;
-    assert { :sourceloc "/Users/schaef/git/jar2bpl/jar2bpl_test/regression/corner_cases/cc01/CornerCases01.java",53,17,53,27 } true;
-    call temp$1030, $exception := int$CornerCases01$getInt$1892(this12, max18);
-    assert { :sourceloc "/Users/schaef/git/jar2bpl/jar2bpl_test/regression/corner_cases/cc01/CornerCases01.java",53,11,53,13 } true;
-    max18 := temp$1030;
-  block43:
-    assert { :sourceloc "/Users/schaef/git/jar2bpl/jar2bpl_test/regression/corner_cases/cc01/CornerCases01.java",53,11,53,13 } true;
-  block41:
-    assert { :sourceloc "/Users/schaef/git/jar2bpl/jar2bpl_test/regression/corner_cases/cc01/CornerCases01.java",53,11,53,13 } true;
-    assert { :sourceloc "/Users/schaef/git/jar2bpl/jar2bpl_test/regression/corner_cases/cc01/CornerCases01.java",54,9,54,19 } true;
-    temp$1131 := index13;
-    assert { :sourceloc "/Users/schaef/git/jar2bpl/jar2bpl_test/regression/corner_cases/cc01/CornerCases01.java",54,9,54,19 } true;
-    temp$1232 := temp$1131 + max18;
-    assert { :sourceloc "/Users/schaef/git/jar2bpl/jar2bpl_test/regression/corner_cases/cc01/CornerCases01.java",54,9,54,13 } true;
-    index13 := temp$1232;
-  block38:
-    assert { :sourceloc "/Users/schaef/git/jar2bpl/jar2bpl_test/regression/corner_cases/cc01/CornerCases01.java",54,9,54,13 } true;
-    assert { :sourceloc "/Users/schaef/git/jar2bpl/jar2bpl_test/regression/corner_cases/cc01/CornerCases01.java",56,7,56,19 } true;
-    $return := index13;
+    assert { :sourceloc "/Users/schaef/git/jar2bpl/jar2bpl_test/regression/true_positives/tp01/InfeasibleCode01.java",84,4,84,8 } true;
     return;
 }
 
 
-implementation int$CornerCases01$getInt$1892($this:ref, $in_parameter__0:int) returns ($return:int, $exception:ref){
+implementation void$InfeasibleCode01$$la$init$ra$$1898($this:ref) returns ($exception:ref){
     
-var i34 : int;    
-var this33 : ref;    
-var temp$035 : int;
-    assume { :sourceloc "/Users/schaef/git/jar2bpl/jar2bpl_test/regression/corner_cases/cc01/CornerCases01.java",-1,-1,-1,-1 } $this != $null;
-    assert { :sourceloc "/Users/schaef/git/jar2bpl/jar2bpl_test/regression/corner_cases/cc01/CornerCases01.java",59,2,62,2 } true;
-    this33 := $this;
-    assert { :sourceloc "/Users/schaef/git/jar2bpl/jar2bpl_test/regression/corner_cases/cc01/CornerCases01.java",59,21,59,25 } true;
-    i34 := $in_parameter__0;
-    assert { :sourceloc "/Users/schaef/git/jar2bpl/jar2bpl_test/regression/corner_cases/cc01/CornerCases01.java",59,21,59,25 } true;
-    temp$035 := 0;
-    assert { :sourceloc "/Users/schaef/git/jar2bpl/jar2bpl_test/regression/corner_cases/cc01/CornerCases01.java",61,3,61,11 } true;
-    $return := temp$035;
-    return;
-}
-
-
-implementation void$CornerCases01$$la$init$ra$$1893($this:ref) returns ($exception:ref){
-    
-var this36 : ref;
-    assume { :sourceloc "/Users/schaef/git/jar2bpl/jar2bpl_test/regression/corner_cases/cc01/CornerCases01.java",-1,-1,-1,-1 } $this != $null;
-    assert { :sourceloc "/Users/schaef/git/jar2bpl/jar2bpl_test/regression/corner_cases/cc01/CornerCases01.java",5,-1,-1,-1 } true;
-    this36 := $this;
-    assert { :sourceloc "/Users/schaef/git/jar2bpl/jar2bpl_test/regression/corner_cases/cc01/CornerCases01.java",5,-1,-1,-1 } true;
-    call $exception := void$java.lang.Object$$la$init$ra$$38(this36);
-    assert { :sourceloc "/Users/schaef/git/jar2bpl/jar2bpl_test/regression/corner_cases/cc01/CornerCases01.java",5,-1,-1,-1 } true;
+var this80 : ref;
+    assume { :sourceloc "/Users/schaef/git/jar2bpl/jar2bpl_test/regression/true_positives/tp01/InfeasibleCode01.java",-1,-1,-1,-1 } $this != $null;
+    assert { :sourceloc "/Users/schaef/git/jar2bpl/jar2bpl_test/regression/true_positives/tp01/InfeasibleCode01.java",7,-1,-1,-1 } true;
+    this80 := $this;
+    assert { :sourceloc "/Users/schaef/git/jar2bpl/jar2bpl_test/regression/true_positives/tp01/InfeasibleCode01.java",7,-1,-1,-1 } true;
+    call $exception := void$java.lang.Object$$la$init$ra$$38(this80);
+    assert { :sourceloc "/Users/schaef/git/jar2bpl/jar2bpl_test/regression/true_positives/tp01/InfeasibleCode01.java",7,-1,-1,-1 } true;
     return;
 }
 
